converted many HOL/Auth theories to Isar scripts

src/HOL/Auth/OtwayRees.thy
@@ -1,44 +1,49 @@
-(*  
+(*  Title:      HOL/Auth/OtwayRees
+    ID:         $Id$
+    Author:     Lawrence C Paulson, Cambridge University Computer Laboratory
+    Copyright   1996  University of Cambridge
+
 Inductive relation "otway" for the Otway-Rees protocol
 extended by Gets primitive.
 
 Version that encrypts Nonce NB
 
+From page 244 of
+  Burrows, Abadi and Needham.  A Logic of Authentication.
+  Proc. Royal Soc. 426 (1989)
 *)
 
-OtwayRees = Shared + 
+theory OtwayRees = Shared:
 
 
-consts  otway   :: event list set
+consts  otway   :: "event list set"
 inductive "otway"
-  intrs 
+  intros
          (*Initial trace is empty*)
-    Nil  "[] \\<in> otway"
-
-         (** These rules allow agents to send messages to themselves **)
+   Nil:  "[] \<in> otway"
 
          (*The spy MAY say anything he CAN say.  We do not expect him to
            invent new nonces here, but he can also use NS1.  Common to
            all similar protocols.*)
-    Fake "[| evsf \\<in> otway;  X \\<in> synth (analz (knows Spy evsf)) |]
-          ==> Says Spy B X  # evsf : otway"
+   Fake: "[| evsf \<in> otway;  X \<in> synth (analz (knows Spy evsf)) |]
+          ==> Says Spy B X  # evsf \<in> otway"
 
          (*A message that has been sent can be received by the
            intended recipient.*)
-    Reception "[| evsr \\<in> otway;  Says A B X : set evsr |]
-               ==> Gets B X # evsr : otway"
+   Reception: "[| evsr \<in> otway;  Says A B X \<in>set evsr |]
+               ==> Gets B X # evsr \<in> otway"
 
          (*Alice initiates a protocol run*)
-    OR1  "[| evs1 \\<in> otway;  Nonce NA \\<notin> used evs1 |]
-          ==> Says A B {|Nonce NA, Agent A, Agent B, 
-                         Crypt (shrK A) {|Nonce NA, Agent A, Agent B|} |} 
+   OR1:  "[| evs1 \<in> otway;  Nonce NA \<notin> used evs1 |]
+          ==> Says A B {|Nonce NA, Agent A, Agent B,
+                         Crypt (shrK A) {|Nonce NA, Agent A, Agent B|} |}
                  # evs1 : otway"
 
          (*Bob's response to Alice's message.  Note that NB is encrypted.*)
-    OR2  "[| evs2 \\<in> otway;  Nonce NB \\<notin> used evs2;
+   OR2:  "[| evs2 \<in> otway;  Nonce NB \<notin> used evs2;
              Gets B {|Nonce NA, Agent A, Agent B, X|} : set evs2 |]
-          ==> Says B Server 
-                  {|Nonce NA, Agent A, Agent B, X, 
+          ==> Says B Server
+                  {|Nonce NA, Agent A, Agent B, X,
                     Crypt (shrK B)
                       {|Nonce NA, Nonce NB, Agent A, Agent B|}|}
                  # evs2 : otway"
@@ -46,23 +51,23 @@ inductive "otway"
          (*The Server receives Bob's message and checks that the three NAs
            match.  Then he sends a new session key to Bob with a packet for
            forwarding to Alice.*)
-    OR3  "[| evs3 \\<in> otway;  Key KAB \\<notin> used evs3;
-             Gets Server 
-                  {|Nonce NA, Agent A, Agent B, 
-                    Crypt (shrK A) {|Nonce NA, Agent A, Agent B|}, 
+   OR3:  "[| evs3 \<in> otway;  Key KAB \<notin> used evs3;
+             Gets Server
+                  {|Nonce NA, Agent A, Agent B,
+                    Crypt (shrK A) {|Nonce NA, Agent A, Agent B|},
                     Crypt (shrK B) {|Nonce NA, Nonce NB, Agent A, Agent B|}|}
                : set evs3 |]
-          ==> Says Server B 
-                  {|Nonce NA, 
+          ==> Says Server B
+                  {|Nonce NA,
                     Crypt (shrK A) {|Nonce NA, Key KAB|},
                     Crypt (shrK B) {|Nonce NB, Key KAB|}|}
                  # evs3 : otway"
 
          (*Bob receives the Server's (?) message and compares the Nonces with
 	   those in the message he previously sent the Server.
-           Need B \\<noteq> Server because we allow messages to self.*)
-    OR4  "[| evs4 \\<in> otway;  B \\<noteq> Server;
-             Says B Server {|Nonce NA, Agent A, Agent B, X', 
+           Need B \<noteq> Server because we allow messages to self.*)
+   OR4:  "[| evs4 \<in> otway;  B \<noteq> Server;
+             Says B Server {|Nonce NA, Agent A, Agent B, X',
                              Crypt (shrK B)
                                    {|Nonce NA, Nonce NB, Agent A, Agent B|}|}
                : set evs4;
@@ -72,9 +77,391 @@ inductive "otway"
 
          (*This message models possible leaks of session keys.  The nonces
            identify the protocol run.*)
-    Oops "[| evso \\<in> otway;  
+   Oops: "[| evso \<in> otway;
              Says Server B {|Nonce NA, X, Crypt (shrK B) {|Nonce NB, Key K|}|}
                : set evso |]
           ==> Notes Spy {|Nonce NA, Nonce NB, Key K|} # evso : otway"
+
+
+declare Says_imp_knows_Spy [THEN analz.Inj, dest]
+declare parts.Body  [dest]
+declare analz_into_parts [dest]
+declare Fake_parts_insert_in_Un  [dest]
+
+
+(*A "possibility property": there are traces that reach the end*)
+lemma "B \<noteq> Server
+      ==> \<exists>K. \<exists>evs \<in> otway.
+             Says B A {|Nonce NA, Crypt (shrK A) {|Nonce NA, Key K|}|}
+               \<in> set evs"
+apply (intro exI bexI)
+apply (rule_tac [2] otway.Nil
+                    [THEN otway.OR1, THEN otway.Reception,
+                     THEN otway.OR2, THEN otway.Reception,
+                     THEN otway.OR3, THEN otway.Reception, THEN otway.OR4])
+apply possibility
+done
+
+lemma Gets_imp_Says [dest!]:
+     "[| Gets B X \<in> set evs; evs \<in> otway |] ==> \<exists>A. Says A B X \<in> set evs"
+apply (erule rev_mp)
+apply (erule otway.induct)
+apply auto
+done
+
+
+(**** Inductive proofs about otway ****)
+
+(** For reasoning about the encrypted portion of messages **)
+
+lemma OR2_analz_knows_Spy:
+     "[| Gets B {|N, Agent A, Agent B, X|} \<in> set evs;  evs \<in> otway |]
+      ==> X \<in> analz (knows Spy evs)"
+by blast
+
+lemma OR4_analz_knows_Spy:
+     "[| Gets B {|N, X, Crypt (shrK B) X'|} \<in> set evs;  evs \<in> otway |]
+      ==> X \<in> analz (knows Spy evs)"
+by blast
+
+(*These lemmas assist simplification by removing forwarded X-variables.
+  We can replace them by rewriting with parts_insert2 and proving using
+  dest: parts_cut, but the proofs become more difficult.*)
+lemmas OR2_parts_knows_Spy =
+    OR2_analz_knows_Spy [THEN analz_into_parts, standard]
+
+(*There could be OR4_parts_knows_Spy and Oops_parts_knows_Spy, but for
+  some reason proofs work without them!*)
+
+
+(** Theorems of the form X \<notin> parts (knows Spy evs) imply that NOBODY
+    sends messages containing X! **)
+
+(*Spy never sees a good agent's shared key!*)
+lemma Spy_see_shrK [simp]:
+     "evs \<in> otway ==> (Key (shrK A) \<in> parts (knows Spy evs)) = (A \<in> bad)"
+apply (erule otway.induct, force,
+       drule_tac [4] OR2_parts_knows_Spy, simp_all)
+apply blast+
+done
+
+lemma Spy_analz_shrK [simp]:
+     "evs \<in> otway ==> (Key (shrK A) \<in> analz (knows Spy evs)) = (A \<in> bad)"
+by auto
+
+lemma Spy_see_shrK_D [dest!]:
+     "[|Key (shrK A) \<in> parts (knows Spy evs);  evs \<in> otway|] ==> A \<in> bad"
+by (blast dest: Spy_see_shrK)
+
+
+(*** Proofs involving analz ***)
+
+(*Describes the form of K and NA when the Server sends this message.  Also
+  for Oops case.*)
+lemma Says_Server_message_form:
+     "[| Says Server B {|NA, X, Crypt (shrK B) {|NB, Key K|}|} \<in> set evs;
+         evs \<in> otway |]
+      ==> K \<notin> range shrK & (\<exists>i. NA = Nonce i) & (\<exists>j. NB = Nonce j)"
+apply (erule rev_mp, erule otway.induct, simp_all)
+apply blast
+done
+
+
+(****
+ The following is to prove theorems of the form
+
+  Key K \<in> analz (insert (Key KAB) (knows Spy evs)) ==>
+  Key K \<in> analz (knows Spy evs)
+
+ A more general formula must be proved inductively.
+****)
+
+
+(** Session keys are not used to encrypt other session keys **)
+
+(*The equality makes the induction hypothesis easier to apply*)
+lemma analz_image_freshK [rule_format]:
+ "evs \<in> otway ==>
+   \<forall>K KK. KK <= -(range shrK) -->
+          (Key K \<in> analz (Key`KK Un (knows Spy evs))) =
+          (K \<in> KK | Key K \<in> analz (knows Spy evs))"
+apply (erule otway.induct, force)
+apply (frule_tac [7] Says_Server_message_form)
+apply (drule_tac [6] OR4_analz_knows_Spy)
+apply (drule_tac [4] OR2_analz_knows_Spy)
+apply analz_freshK
+apply spy_analz
+done
+
+
+lemma analz_insert_freshK:
+  "[| evs \<in> otway;  KAB \<notin> range shrK |] ==>
+      Key K \<in> analz (insert (Key KAB) (knows Spy evs)) =
+      (K = KAB | Key K \<in> analz (knows Spy evs))"
+by (simp only: analz_image_freshK analz_image_freshK_simps)
+
+
+(*** The Key K uniquely identifies the Server's  message. **)
+
+lemma unique_session_keys:
+     "[| Says Server B {|NA, X, Crypt (shrK B) {|NB, K|}|}   \<in> set evs;
+         Says Server B' {|NA',X',Crypt (shrK B') {|NB',K|}|} \<in> set evs;
+         evs \<in> otway |] ==> X=X' & B=B' & NA=NA' & NB=NB'"
+apply (erule rev_mp)
+apply (erule rev_mp)
+apply (erule otway.induct, simp_all)
+(*Remaining cases: OR3 and OR4*)
+apply blast+
+done
+
+
+(**** Authenticity properties relating to NA ****)
+
+(*Only OR1 can have caused such a part of a message to appear.*)
+lemma Crypt_imp_OR1 [rule_format]:
+ "[| A \<notin> bad;  evs \<in> otway |]
+  ==> Crypt (shrK A) {|NA, Agent A, Agent B|} \<in> parts (knows Spy evs) -->
+      Says A B {|NA, Agent A, Agent B,
+                 Crypt (shrK A) {|NA, Agent A, Agent B|}|}
+        \<in> set evs"
+apply (erule otway.induct, force,
+       drule_tac [4] OR2_parts_knows_Spy, simp_all)
+apply blast+
+done
+
+lemma Crypt_imp_OR1_Gets:
+     "[| Gets B {|NA, Agent A, Agent B,
+                  Crypt (shrK A) {|NA, Agent A, Agent B|}|} \<in> set evs;
+         A \<notin> bad; evs \<in> otway |]
+       ==> Says A B {|NA, Agent A, Agent B,
+                      Crypt (shrK A) {|NA, Agent A, Agent B|}|}
+             \<in> set evs"
+by (blast dest: Crypt_imp_OR1)
+
+
+(** The Nonce NA uniquely identifies A's message. **)
+
+lemma unique_NA:
+     "[| Crypt (shrK A) {|NA, Agent A, Agent B|} \<in> parts (knows Spy evs);
+         Crypt (shrK A) {|NA, Agent A, Agent C|} \<in> parts (knows Spy evs);
+         evs \<in> otway;  A \<notin> bad |]
+      ==> B = C"
+apply (erule rev_mp, erule rev_mp)
+apply (erule otway.induct, force,
+       drule_tac [4] OR2_parts_knows_Spy, simp_all)
+apply blast+
+done
+
+
+(*It is impossible to re-use a nonce in both OR1 and OR2.  This holds because
+  OR2 encrypts Nonce NB.  It prevents the attack that can occur in the
+  over-simplified version of this protocol: see OtwayRees_Bad.*)
+lemma no_nonce_OR1_OR2:
+   "[| Crypt (shrK A) {|NA, Agent A, Agent B|} \<in> parts (knows Spy evs);
+       A \<notin> bad;  evs \<in> otway |]
+    ==> Crypt (shrK A) {|NA', NA, Agent A', Agent A|} \<notin> parts (knows Spy evs)"
+apply (erule rev_mp)
+apply (erule otway.induct, force,
+       drule_tac [4] OR2_parts_knows_Spy, simp_all)
+apply blast+
+done
+
+(*Crucial property: If the encrypted message appears, and A has used NA
+  to start a run, then it originated with the Server!*)
+lemma NA_Crypt_imp_Server_msg [rule_format]:
+     "[| A \<notin> bad;  evs \<in> otway |]
+      ==> Says A B {|NA, Agent A, Agent B,
+                     Crypt (shrK A) {|NA, Agent A, Agent B|}|} \<in> set evs -->
+          Crypt (shrK A) {|NA, Key K|} \<in> parts (knows Spy evs)
+          --> (\<exists>NB. Says Server B
+                         {|NA,
+                           Crypt (shrK A) {|NA, Key K|},
+                           Crypt (shrK B) {|NB, Key K|}|} \<in> set evs)"
+apply (erule otway.induct, force,
+       drule_tac [4] OR2_parts_knows_Spy, simp_all)
+apply blast
+(*OR1: it cannot be a new Nonce, contradiction.*)
+apply blast
+(*OR3*)
+apply (blast dest!: no_nonce_OR1_OR2 intro: unique_NA)
+(*OR4*)
+apply (blast intro!: Crypt_imp_OR1)
+done
+
+
+(*Corollary: if A receives B's OR4 message and the nonce NA agrees
+  then the key really did come from the Server!  CANNOT prove this of the
+  bad form of this protocol, even though we can prove
+  Spy_not_see_encrypted_key*)
+lemma A_trusts_OR4:
+     "[| Says A  B {|NA, Agent A, Agent B,
+                     Crypt (shrK A) {|NA, Agent A, Agent B|}|} \<in> set evs;
+         Says B' A {|NA, Crypt (shrK A) {|NA, Key K|}|} \<in> set evs;
+     A \<notin> bad;  evs \<in> otway |]
+  ==> \<exists>NB. Says Server B
+               {|NA,
+                 Crypt (shrK A) {|NA, Key K|},
+                 Crypt (shrK B) {|NB, Key K|}|}
+                 \<in> set evs"
+by (blast intro!: NA_Crypt_imp_Server_msg)
+
+
+(** Crucial secrecy property: Spy does not see the keys sent in msg OR3
+    Does not in itself guarantee security: an attack could violate
+    the premises, e.g. by having A=Spy **)
+
+lemma secrecy_lemma:
+ "[| A \<notin> bad;  B \<notin> bad;  evs \<in> otway |]
+  ==> Says Server B
+        {|NA, Crypt (shrK A) {|NA, Key K|},
+          Crypt (shrK B) {|NB, Key K|}|} \<in> set evs -->
+      Notes Spy {|NA, NB, Key K|} \<notin> set evs -->
+      Key K \<notin> analz (knows Spy evs)"
+apply (erule otway.induct, force)
+apply (frule_tac [7] Says_Server_message_form)
+apply (drule_tac [6] OR4_analz_knows_Spy)
+apply (drule_tac [4] OR2_analz_knows_Spy)
+apply (simp_all add: analz_insert_eq analz_insert_freshK pushes)
+apply spy_analz  (*Fake*)
+(*OR3, OR4, Oops*)
+apply (blast dest: unique_session_keys)+
+done
+
+lemma Spy_not_see_encrypted_key:
+     "[| Says Server B
+          {|NA, Crypt (shrK A) {|NA, Key K|},
+                Crypt (shrK B) {|NB, Key K|}|} \<in> set evs;
+         Notes Spy {|NA, NB, Key K|} \<notin> set evs;
+         A \<notin> bad;  B \<notin> bad;  evs \<in> otway |]
+      ==> Key K \<notin> analz (knows Spy evs)"
+by (blast dest: Says_Server_message_form secrecy_lemma)
+
+
+(*A's guarantee.  The Oops premise quantifies over NB because A cannot know
+  what it is.*)
+lemma A_gets_good_key:
+     "[| Says A  B {|NA, Agent A, Agent B,
+                     Crypt (shrK A) {|NA, Agent A, Agent B|}|} \<in> set evs;
+         Says B' A {|NA, Crypt (shrK A) {|NA, Key K|}|} \<in> set evs;
+         \<forall>NB. Notes Spy {|NA, NB, Key K|} \<notin> set evs;
+         A \<notin> bad;  B \<notin> bad;  evs \<in> otway |]
+      ==> Key K \<notin> analz (knows Spy evs)"
+by (blast dest!: A_trusts_OR4 Spy_not_see_encrypted_key)
+
+
+
+(**** Authenticity properties relating to NB ****)
+
+(*Only OR2 can have caused such a part of a message to appear.  We do not
+  know anything about X: it does NOT have to have the right form.*)
+lemma Crypt_imp_OR2:
+     "[| Crypt (shrK B) {|NA, NB, Agent A, Agent B|} \<in> parts (knows Spy evs);
+         B \<notin> bad;  evs \<in> otway |]
+      ==> \<exists>X. Says B Server
+                 {|NA, Agent A, Agent B, X,
+                   Crypt (shrK B) {|NA, NB, Agent A, Agent B|}|}
+                 \<in> set evs"
+apply (erule rev_mp)
+apply (erule otway.induct, force,
+       drule_tac [4] OR2_parts_knows_Spy, simp_all)
+apply blast+
+done
+
+
+(** The Nonce NB uniquely identifies B's  message. **)
+
+lemma unique_NB:
+     "[| Crypt (shrK B) {|NA, NB, Agent A, Agent B|} \<in> parts(knows Spy evs);
+         Crypt (shrK B) {|NC, NB, Agent C, Agent B|} \<in> parts(knows Spy evs);
+           evs \<in> otway;  B \<notin> bad |]
+         ==> NC = NA & C = A"
+apply (erule rev_mp, erule rev_mp)
+apply (erule otway.induct, force,
+       drule_tac [4] OR2_parts_knows_Spy, simp_all)
+(*Fake, OR2*)
+apply blast+
+done
+
+(*If the encrypted message appears, and B has used Nonce NB,
+  then it originated with the Server!  Quite messy proof.*)
+lemma NB_Crypt_imp_Server_msg [rule_format]:
+ "[| B \<notin> bad;  evs \<in> otway |]
+  ==> Crypt (shrK B) {|NB, Key K|} \<in> parts (knows Spy evs)
+      --> (\<forall>X'. Says B Server
+                     {|NA, Agent A, Agent B, X',
+                       Crypt (shrK B) {|NA, NB, Agent A, Agent B|}|}
+           \<in> set evs
+           --> Says Server B
+                {|NA, Crypt (shrK A) {|NA, Key K|},
+                      Crypt (shrK B) {|NB, Key K|}|}
+                    \<in> set evs)"
+apply simp
+apply (erule otway.induct, force,
+       drule_tac [4] OR2_parts_knows_Spy, simp_all)
+apply blast
+(*OR1: it cannot be a new Nonce, contradiction.*)
+(*OR2*)
+apply blast
+(*OR3: needs elim: MPair_parts or it takes forever!*)
+apply (blast dest: unique_NB dest!: no_nonce_OR1_OR2)
+(*OR4*)
+apply (blast dest!: Crypt_imp_OR2)
+done
+
+
+(*Guarantee for B: if it gets a message with matching NB then the Server
+  has sent the correct message.*)
+lemma B_trusts_OR3:
+     "[| Says B Server {|NA, Agent A, Agent B, X',
+                         Crypt (shrK B) {|NA, NB, Agent A, Agent B|} |}
+           \<in> set evs;
+         Gets B {|NA, X, Crypt (shrK B) {|NB, Key K|}|} \<in> set evs;
+         B \<notin> bad;  evs \<in> otway |]
+      ==> Says Server B
+               {|NA,
+                 Crypt (shrK A) {|NA, Key K|},
+                 Crypt (shrK B) {|NB, Key K|}|}
+                 \<in> set evs"
+by (blast intro!: NB_Crypt_imp_Server_msg)
+
+
+(*The obvious combination of B_trusts_OR3 with Spy_not_see_encrypted_key*)
+lemma B_gets_good_key:
+     "[| Says B Server {|NA, Agent A, Agent B, X',
+                         Crypt (shrK B) {|NA, NB, Agent A, Agent B|} |}
+           \<in> set evs;
+         Gets B {|NA, X, Crypt (shrK B) {|NB, Key K|}|} \<in> set evs;
+         Notes Spy {|NA, NB, Key K|} \<notin> set evs;
+         A \<notin> bad;  B \<notin> bad;  evs \<in> otway |]
+      ==> Key K \<notin> analz (knows Spy evs)"
+by (blast dest!: B_trusts_OR3 Spy_not_see_encrypted_key)
+
+
+lemma OR3_imp_OR2:
+     "[| Says Server B
+              {|NA, Crypt (shrK A) {|NA, Key K|},
+                Crypt (shrK B) {|NB, Key K|}|} \<in> set evs;
+         B \<notin> bad;  evs \<in> otway |]
+  ==> \<exists>X. Says B Server {|NA, Agent A, Agent B, X,
+                            Crypt (shrK B) {|NA, NB, Agent A, Agent B|} |}
+              \<in> set evs"
+apply (erule rev_mp)
+apply (erule otway.induct, simp_all)
+apply (blast dest!: Crypt_imp_OR2)+
+done
+
+
+(*After getting and checking OR4, agent A can trust that B has been active.
+  We could probably prove that X has the expected form, but that is not
+  strictly necessary for authentication.*)
+lemma A_auths_B:
+     "[| Says B' A {|NA, Crypt (shrK A) {|NA, Key K|}|} \<in> set evs;
+         Says A  B {|NA, Agent A, Agent B,
+                     Crypt (shrK A) {|NA, Agent A, Agent B|}|} \<in> set evs;
+         A \<notin> bad;  B \<notin> bad;  evs \<in> otway |]
+  ==> \<exists>NB X. Says B Server {|NA, Agent A, Agent B, X,
+                               Crypt (shrK B)  {|NA, NB, Agent A, Agent B|} |}
+                 \<in> set evs"
+by (blast dest!: A_trusts_OR4 OR3_imp_OR2)
 
 end
