src/HOL/Auth/OtwayRees_AN.thy
@@ -5,7 +5,7 @@
 
 Inductive relation "otway" for the Otway-Rees protocol.
 
-Simplified version with minimal encryption but explicit messages
+Abadi-Needham simplified version: minimal encryption, explicit messages
 
 Note that the formalization does not even assume that nonces are fresh.
 This is because the protocol does not rely on uniqueness of nonces for
@@ -17,61 +17,298 @@ From page 11 of
   IEEE Trans. SE 22 (1), 1996
 *)
 
-OtwayRees_AN = Shared + 
+theory OtwayRees_AN = Shared:
 
-consts  otway   :: event list set
+consts  otway   :: "event list set"
 inductive "otway"
-  intrs 
+  intros
          (*Initial trace is empty*)
-    Nil  "[]: otway"
+   Nil:  "[] \<in> otway"
 
          (*The spy MAY say anything he CAN say.  We do not expect him to
            invent new nonces here, but he can also use NS1.  Common to
            all similar protocols.*)
-    Fake "[| evs \\<in> otway;  X \\<in> synth (analz (knows Spy evs)) |]
-          ==> Says Spy B X  # evs \\<in> otway"
+   Fake: "[| evsf \<in> otway;  X \<in> synth (analz (knows Spy evsf)) |]
+          ==> Says Spy B X  # evsf \<in> otway"
 
          (*A message that has been sent can be received by the
            intended recipient.*)
-    Reception "[| evsr \\<in> otway;  Says A B X \\<in>set evsr |]
-               ==> Gets B X # evsr \\<in> otway"
+   Reception: "[| evsr \<in> otway;  Says A B X \<in>set evsr |]
+               ==> Gets B X # evsr \<in> otway"
 
          (*Alice initiates a protocol run*)
-    OR1  "[| evs1 \\<in> otway |]
-          ==> Says A B {|Agent A, Agent B, Nonce NA|} # evs1 \\<in> otway"
+   OR1:  "evs1 \<in> otway
+          ==> Says A B {|Agent A, Agent B, Nonce NA|} # evs1 \<in> otway"
 
          (*Bob's response to Alice's message.*)
-    OR2  "[| evs2 \\<in> otway;  
-             Gets B {|Agent A, Agent B, Nonce NA|} \\<in>set evs2 |]
+   OR2:  "[| evs2 \<in> otway;
+             Gets B {|Agent A, Agent B, Nonce NA|} \<in>set evs2 |]
           ==> Says B Server {|Agent A, Agent B, Nonce NA, Nonce NB|}
-                 # evs2 \\<in> otway"
+                 # evs2 \<in> otway"
 
          (*The Server receives Bob's message.  Then he sends a new
            session key to Bob with a packet for forwarding to Alice.*)
-    OR3  "[| evs3 \\<in> otway;  Key KAB \\<notin> used evs3;
+   OR3:  "[| evs3 \<in> otway;  Key KAB \<notin> used evs3;
              Gets Server {|Agent A, Agent B, Nonce NA, Nonce NB|}
-               \\<in>set evs3 |]
-          ==> Says Server B 
+               \<in>set evs3 |]
+          ==> Says Server B
                {|Crypt (shrK A) {|Nonce NA, Agent A, Agent B, Key KAB|},
                  Crypt (shrK B) {|Nonce NB, Agent A, Agent B, Key KAB|}|}
-              # evs3 \\<in> otway"
+              # evs3 \<in> otway"
 
          (*Bob receives the Server's (?) message and compares the Nonces with
 	   those in the message he previously sent the Server.
-           Need B \\<noteq> Server because we allow messages to self.*)
-    OR4  "[| evs4 \\<in> otway;  B \\<noteq> Server; 
-             Says B Server {|Agent A, Agent B, Nonce NA, Nonce NB|} \\<in>set evs4;
+           Need B \<noteq> Server because we allow messages to self.*)
+   OR4:  "[| evs4 \<in> otway;  B \<noteq> Server;
+             Says B Server {|Agent A, Agent B, Nonce NA, Nonce NB|} \<in>set evs4;
              Gets B {|X, Crypt(shrK B){|Nonce NB,Agent A,Agent B,Key K|}|}
-               \\<in>set evs4 |]
-          ==> Says B A X # evs4 \\<in> otway"
+               \<in>set evs4 |]
+          ==> Says B A X # evs4 \<in> otway"
 
          (*This message models possible leaks of session keys.  The nonces
            identify the protocol run.  B is not assumed to know shrK A.*)
-    Oops "[| evso \\<in> otway;  
-             Says Server B 
-                      {|Crypt (shrK A) {|Nonce NA, Agent A, Agent B, Key K|}, 
+   Oops: "[| evso \<in> otway;
+             Says Server B
+                      {|Crypt (shrK A) {|Nonce NA, Agent A, Agent B, Key K|},
                         Crypt (shrK B) {|Nonce NB, Agent A, Agent B, Key K|}|}
-               \\<in>set evso |]
-          ==> Notes Spy {|Nonce NA, Nonce NB, Key K|} # evso \\<in> otway"
+               \<in>set evso |]
+          ==> Notes Spy {|Nonce NA, Nonce NB, Key K|} # evso \<in> otway"
+
+
+declare Says_imp_knows_Spy [THEN analz.Inj, dest]
+declare parts.Body  [dest]
+declare analz_into_parts [dest]
+declare Fake_parts_insert_in_Un  [dest]
+
+
+(*A "possibility property": there are traces that reach the end*)
+lemma "B \<noteq> Server
+      ==> \<exists>K. \<exists>evs \<in> otway.
+           Says B A (Crypt (shrK A) {|Nonce NA, Agent A, Agent B, Key K|})
+             \<in> set evs"
+apply (intro exI bexI)
+apply (rule_tac [2] otway.Nil
+                    [THEN otway.OR1, THEN otway.Reception,
+                     THEN otway.OR2, THEN otway.Reception,
+                     THEN otway.OR3, THEN otway.Reception, THEN otway.OR4])
+apply possibility
+done
+
+lemma Gets_imp_Says [dest!]:
+     "[| Gets B X \<in> set evs; evs \<in> otway |] ==> \<exists>A. Says A B X \<in> set evs"
+by (erule rev_mp, erule otway.induct, auto)
+
+
+(**** Inductive proofs about otway ****)
+
+(** For reasoning about the encrypted portion of messages **)
+
+lemma OR4_analz_knows_Spy:
+     "[| Gets B {|X, Crypt(shrK B) X'|} \<in> set evs;  evs \<in> otway |]
+      ==> X \<in> analz (knows Spy evs)"
+by blast
+
+
+(** Theorems of the form X \<notin> parts (knows Spy evs) imply that NOBODY
+    sends messages containing X! **)
+
+(*Spy never sees a good agent's shared key!*)
+lemma Spy_see_shrK [simp]:
+     "evs \<in> otway ==> (Key (shrK A) \<in> parts (knows Spy evs)) = (A \<in> bad)"
+apply (erule otway.induct, simp_all)
+apply blast+
+done
+
+lemma Spy_analz_shrK [simp]:
+     "evs \<in> otway ==> (Key (shrK A) \<in> analz (knows Spy evs)) = (A \<in> bad)"
+by auto
+
+lemma Spy_see_shrK_D [dest!]:
+     "[|Key (shrK A) \<in> parts (knows Spy evs);  evs \<in> otway|] ==> A \<in> bad"
+by (blast dest: Spy_see_shrK)
+
+
+(*** Proofs involving analz ***)
+
+(*Describes the form of K and NA when the Server sends this message.*)
+lemma Says_Server_message_form:
+     "[| Says Server B
+            {|Crypt (shrK A) {|NA, Agent A, Agent B, Key K|},
+              Crypt (shrK B) {|NB, Agent A, Agent B, Key K|}|}
+           \<in> set evs;
+         evs \<in> otway |]
+      ==> K \<notin> range shrK & (\<exists>i. NA = Nonce i) & (\<exists>j. NB = Nonce j)"
+apply (erule rev_mp)
+apply (erule otway.induct)
+apply simp_all
+apply blast
+done
+
+
+
+(****
+ The following is to prove theorems of the form
+
+  Key K \<in> analz (insert (Key KAB) (knows Spy evs)) ==>
+  Key K \<in> analz (knows Spy evs)
+
+ A more general formula must be proved inductively.
+****)
+
+
+(** Session keys are not used to encrypt other session keys **)
+
+(*The equality makes the induction hypothesis easier to apply*)
+lemma analz_image_freshK [rule_format]:
+ "evs \<in> otway ==>
+   \<forall>K KK. KK <= -(range shrK) -->
+          (Key K \<in> analz (Key`KK Un (knows Spy evs))) =
+          (K \<in> KK | Key K \<in> analz (knows Spy evs))"
+apply (erule otway.induct, force)
+apply (frule_tac [7] Says_Server_message_form)
+apply (drule_tac [6] OR4_analz_knows_Spy)
+apply analz_freshK
+apply spy_analz
+done
+
+lemma analz_insert_freshK:
+  "[| evs \<in> otway;  KAB \<notin> range shrK |] ==>
+      Key K \<in> analz (insert (Key KAB) (knows Spy evs)) =
+      (K = KAB | Key K \<in> analz (knows Spy evs))"
+by (simp only: analz_image_freshK analz_image_freshK_simps)
+
+
+(*** The Key K uniquely identifies the Server's message. **)
+
+lemma unique_session_keys:
+     "[| Says Server B
+          {|Crypt (shrK A) {|NA, Agent A, Agent B, K|},
+            Crypt (shrK B) {|NB, Agent A, Agent B, K|}|}
+         \<in> set evs;
+        Says Server B'
+          {|Crypt (shrK A') {|NA', Agent A', Agent B', K|},
+            Crypt (shrK B') {|NB', Agent A', Agent B', K|}|}
+         \<in> set evs;
+        evs \<in> otway |]
+     ==> A=A' & B=B' & NA=NA' & NB=NB'"
+apply (erule rev_mp, erule rev_mp, erule otway.induct)
+apply simp_all
+(*Remaining cases: OR3 and OR4*)
+apply blast+
+done
+
+
+(**** Authenticity properties relating to NA ****)
+
+(*If the encrypted message appears then it originated with the Server!*)
+lemma NA_Crypt_imp_Server_msg [rule_format]:
+    "[| A \<notin> bad;  A \<noteq> B;  evs \<in> otway |]
+     ==> Crypt (shrK A) {|NA, Agent A, Agent B, Key K|} \<in> parts (knows Spy evs)
+       --> (\<exists>NB. Says Server B
+                    {|Crypt (shrK A) {|NA, Agent A, Agent B, Key K|},
+                      Crypt (shrK B) {|NB, Agent A, Agent B, Key K|}|}
+                    \<in> set evs)"
+apply (erule otway.induct, force)
+apply (simp_all add: ex_disj_distrib)
+(*Fake, OR3*)
+apply blast+;
+done
+
+
+(*Corollary: if A receives B's OR4 message then it originated with the Server.
+  Freshness may be inferred from nonce NA.*)
+lemma A_trusts_OR4:
+     "[| Says B' A (Crypt (shrK A) {|NA, Agent A, Agent B, Key K|}) \<in> set evs;
+         A \<notin> bad;  A \<noteq> B;  evs \<in> otway |]
+      ==> \<exists>NB. Says Server B
+                  {|Crypt (shrK A) {|NA, Agent A, Agent B, Key K|},
+                    Crypt (shrK B) {|NB, Agent A, Agent B, Key K|}|}
+                 \<in> set evs"
+by (blast intro!: NA_Crypt_imp_Server_msg)
+
+
+(** Crucial secrecy property: Spy does not see the keys sent in msg OR3
+    Does not in itself guarantee security: an attack could violate
+    the premises, e.g. by having A=Spy **)
+
+lemma secrecy_lemma:
+     "[| A \<notin> bad;  B \<notin> bad;  evs \<in> otway |]
+      ==> Says Server B
+           {|Crypt (shrK A) {|NA, Agent A, Agent B, Key K|},
+             Crypt (shrK B) {|NB, Agent A, Agent B, Key K|}|}
+          \<in> set evs -->
+          Notes Spy {|NA, NB, Key K|} \<notin> set evs -->
+          Key K \<notin> analz (knows Spy evs)"
+apply (erule otway.induct, force)
+apply (frule_tac [7] Says_Server_message_form)
+apply (drule_tac [6] OR4_analz_knows_Spy)
+apply (simp_all add: analz_insert_eq analz_insert_freshK pushes)
+apply spy_analz  (*Fake*)
+(*OR3, OR4, Oops*)
+apply (blast dest: unique_session_keys)+
+done
+
+
+lemma Spy_not_see_encrypted_key:
+     "[| Says Server B
+            {|Crypt (shrK A) {|NA, Agent A, Agent B, Key K|},
+              Crypt (shrK B) {|NB, Agent A, Agent B, Key K|}|}
+           \<in> set evs;
+         Notes Spy {|NA, NB, Key K|} \<notin> set evs;
+         A \<notin> bad;  B \<notin> bad;  evs \<in> otway |]
+      ==> Key K \<notin> analz (knows Spy evs)"
+by (blast dest: Says_Server_message_form secrecy_lemma)
+
+
+(*A's guarantee.  The Oops premise quantifies over NB because A cannot know
+  what it is.*)
+lemma A_gets_good_key:
+     "[| Says B' A (Crypt (shrK A) {|NA, Agent A, Agent B, Key K|}) \<in> set evs;
+         \<forall>NB. Notes Spy {|NA, NB, Key K|} \<notin> set evs;
+         A \<notin> bad;  B \<notin> bad;  A \<noteq> B;  evs \<in> otway |]
+      ==> Key K \<notin> analz (knows Spy evs)"
+by (blast dest!: A_trusts_OR4 Spy_not_see_encrypted_key)
+
+
+
+(**** Authenticity properties relating to NB ****)
+
+(*If the encrypted message appears then it originated with the Server!*)
+
+lemma NB_Crypt_imp_Server_msg [rule_format]:
+ "[| B \<notin> bad;  A \<noteq> B;  evs \<in> otway |]
+  ==> Crypt (shrK B) {|NB, Agent A, Agent B, Key K|} \<in> parts (knows Spy evs)
+      --> (\<exists>NA. Says Server B
+                   {|Crypt (shrK A) {|NA, Agent A, Agent B, Key K|},
+                     Crypt (shrK B) {|NB, Agent A, Agent B, Key K|}|}
+                   \<in> set evs)"
+apply (erule otway.induct, force, simp_all add: ex_disj_distrib)
+(*Fake, OR3*)
+apply blast+;
+done
+
+
+
+(*Guarantee for B: if it gets a well-formed certificate then the Server
+  has sent the correct message in round 3.*)
+lemma B_trusts_OR3:
+     "[| Says S B {|X, Crypt (shrK B) {|NB, Agent A, Agent B, Key K|}|}
+           \<in> set evs;
+         B \<notin> bad;  A \<noteq> B;  evs \<in> otway |]
+      ==> \<exists>NA. Says Server B
+                   {|Crypt (shrK A) {|NA, Agent A, Agent B, Key K|},
+                     Crypt (shrK B) {|NB, Agent A, Agent B, Key K|}|}
+                   \<in> set evs"
+by (blast intro!: NB_Crypt_imp_Server_msg)
+
+
+(*The obvious combination of B_trusts_OR3 with Spy_not_see_encrypted_key*)
+lemma B_gets_good_key:
+     "[| Gets B {|X, Crypt (shrK B) {|NB, Agent A, Agent B, Key K|}|}
+          \<in> set evs;
+         \<forall>NA. Notes Spy {|NA, NB, Key K|} \<notin> set evs;
+         A \<notin> bad;  B \<notin> bad;  A \<noteq> B;  evs \<in> otway |]
+      ==> Key K \<notin> analz (knows Spy evs)"
+by (blast dest: B_trusts_OR3 Spy_not_see_encrypted_key)
 
 end
