src/HOL/Auth/WooLam.thy
@@ -14,52 +14,166 @@ Note: this differs from the Woo-Lam protocol discussed by Lowe in his paper
   Computer Security Foundations Workshop, 1996.
 *)
 
-WooLam = Shared + 
+theory WooLam = Shared:
 
-consts  woolam  :: event list set
+consts  woolam  :: "event list set"
 inductive woolam
-  intrs 
+  intros
          (*Initial trace is empty*)
-    Nil  "[] \\<in> woolam"
+   Nil:  "[] \<in> woolam"
 
          (** These rules allow agents to send messages to themselves **)
 
          (*The spy MAY say anything he CAN say.  We do not expect him to
            invent new nonces here, but he can also use NS1.  Common to
            all similar protocols.*)
-    Fake "[| evsf \\<in> woolam;  X \\<in> synth (analz (spies evsf)) |]
-          ==> Says Spy B X  # evsf \\<in> woolam"
+   Fake: "[| evsf \<in> woolam;  X \<in> synth (analz (spies evsf)) |]
+          ==> Says Spy B X  # evsf \<in> woolam"
 
          (*Alice initiates a protocol run*)
-    WL1  "[| evs1 \\<in> woolam |]
-          ==> Says A B (Agent A) # evs1 \\<in> woolam"
+   WL1:  "evs1 \<in> woolam ==> Says A B (Agent A) # evs1 \<in> woolam"
 
          (*Bob responds to Alice's message with a challenge.*)
-    WL2  "[| evs2 \\<in> woolam;  Says A' B (Agent A) \\<in> set evs2 |]
-          ==> Says B A (Nonce NB) # evs2 \\<in> woolam"
+   WL2:  "[| evs2 \<in> woolam;  Says A' B (Agent A) \<in> set evs2 |]
+          ==> Says B A (Nonce NB) # evs2 \<in> woolam"
 
          (*Alice responds to Bob's challenge by encrypting NB with her key.
            B is *not* properly determined -- Alice essentially broadcasts
            her reply.*)
-    WL3  "[| evs3 \\<in> woolam;
-             Says A  B (Agent A)  \\<in> set evs3;
-             Says B' A (Nonce NB) \\<in> set evs3 |]
-          ==> Says A B (Crypt (shrK A) (Nonce NB)) # evs3 \\<in> woolam"
+   WL3:  "[| evs3 \<in> woolam;
+             Says A  B (Agent A)  \<in> set evs3;
+             Says B' A (Nonce NB) \<in> set evs3 |]
+          ==> Says A B (Crypt (shrK A) (Nonce NB)) # evs3 \<in> woolam"
 
          (*Bob forwards Alice's response to the Server.  NOTE: usually
            the messages are shown in chronological order, for clarity.
            But here, exchanging the two events would cause the lemma
            WL4_analz_spies to pick up the wrong assumption!*)
-    WL4  "[| evs4 \\<in> woolam;  
-             Says A'  B X         \\<in> set evs4;
-             Says A'' B (Agent A) \\<in> set evs4 |]
-          ==> Says B Server {|Agent A, Agent B, X|} # evs4 \\<in> woolam"
+   WL4:  "[| evs4 \<in> woolam;
+             Says A'  B X         \<in> set evs4;
+             Says A'' B (Agent A) \<in> set evs4 |]
+          ==> Says B Server {|Agent A, Agent B, X|} # evs4 \<in> woolam"
 
          (*Server decrypts Alice's response for Bob.*)
-    WL5  "[| evs5 \\<in> woolam;  
+   WL5:  "[| evs5 \<in> woolam;
              Says B' Server {|Agent A, Agent B, Crypt (shrK A) (Nonce NB)|}
-               \\<in> set evs5 |]
+               \<in> set evs5 |]
           ==> Says Server B (Crypt (shrK B) {|Agent A, Nonce NB|})
-                 # evs5 \\<in> woolam"
+                 # evs5 \<in> woolam"
+
+
+declare Says_imp_knows_Spy [THEN analz.Inj, dest]
+declare parts.Body  [dest]
+declare analz_into_parts [dest]
+declare Fake_parts_insert_in_Un  [dest]
+
+
+(*A "possibility property": there are traces that reach the end*)
+lemma "\<exists>NB. \<exists>evs \<in> woolam.
+             Says Server B (Crypt (shrK B) {|Agent A, Nonce NB|}) \<in> set evs"
+apply (intro exI bexI)
+apply (rule_tac [2] woolam.Nil
+                    [THEN woolam.WL1, THEN woolam.WL2, THEN woolam.WL3,
+                     THEN woolam.WL4, THEN woolam.WL5])
+apply possibility
+done
+
+(*Could prove forwarding lemmas for WL4, but we do not need them!*)
+
+(**** Inductive proofs about woolam ****)
+
+(** Theorems of the form X \<notin> parts (spies evs) imply that NOBODY
+    sends messages containing X! **)
+
+(*Spy never sees a good agent's shared key!*)
+lemma Spy_see_shrK [simp]:
+     "evs \<in> woolam ==> (Key (shrK A) \<in> parts (spies evs)) = (A \<in> bad)"
+apply (erule woolam.induct, force, simp_all)
+apply blast+
+done
+
+lemma Spy_analz_shrK [simp]:
+     "evs \<in> woolam ==> (Key (shrK A) \<in> analz (spies evs)) = (A \<in> bad)"
+by auto
+
+lemma Spy_see_shrK_D [dest!]:
+     "[|Key (shrK A) \<in> parts (knows Spy evs);  evs \<in> woolam|] ==> A \<in> bad"
+by (blast dest: Spy_see_shrK)
+
+
+(**** Autheticity properties for Woo-Lam ****)
+
+(*** WL4 ***)
+
+(*If the encrypted message appears then it originated with Alice*)
+lemma NB_Crypt_imp_Alice_msg:
+     "[| Crypt (shrK A) (Nonce NB) \<in> parts (spies evs);
+         A \<notin> bad;  evs \<in> woolam |]
+      ==> \<exists>B. Says A B (Crypt (shrK A) (Nonce NB)) \<in> set evs"
+apply (erule rev_mp, erule woolam.induct, force, simp_all)
+apply blast+
+done
+
+(*Guarantee for Server: if it gets a message containing a certificate from
+  Alice, then she originated that certificate.  But we DO NOT know that B
+  ever saw it: the Spy may have rerouted the message to the Server.*)
+lemma Server_trusts_WL4 [dest]:
+     "[| Says B' Server {|Agent A, Agent B, Crypt (shrK A) (Nonce NB)|}
+           \<in> set evs;
+         A \<notin> bad;  evs \<in> woolam |]
+      ==> \<exists>B. Says A B (Crypt (shrK A) (Nonce NB)) \<in> set evs"
+by (blast intro!: NB_Crypt_imp_Alice_msg)
+
+
+(*** WL5 ***)
+
+(*Server sent WL5 only if it received the right sort of message*)
+lemma Server_sent_WL5 [dest]:
+     "[| Says Server B (Crypt (shrK B) {|Agent A, NB|}) \<in> set evs;
+         evs \<in> woolam |]
+      ==> \<exists>B'. Says B' Server {|Agent A, Agent B, Crypt (shrK A) NB|}
+             \<in> set evs"
+apply (erule rev_mp, erule woolam.induct, force, simp_all)
+apply blast+
+done
+
+(*If the encrypted message appears then it originated with the Server!*)
+lemma NB_Crypt_imp_Server_msg [rule_format]:
+     "[| Crypt (shrK B) {|Agent A, NB|} \<in> parts (spies evs);
+         B \<notin> bad;  evs \<in> woolam |]
+      ==> Says Server B (Crypt (shrK B) {|Agent A, NB|}) \<in> set evs"
+apply (erule rev_mp, erule woolam.induct, force, simp_all)
+apply blast+
+done
+
+(*Guarantee for B.  If B gets the Server's certificate then A has encrypted
+  the nonce using her key.  This event can be no older than the nonce itself.
+  But A may have sent the nonce to some other agent and it could have reached
+  the Server via the Spy.*)
+lemma B_trusts_WL5:
+     "[| Says S B (Crypt (shrK B) {|Agent A, Nonce NB|}): set evs;
+         A \<notin> bad;  B \<notin> bad;  evs \<in> woolam  |]
+      ==> \<exists>B. Says A B (Crypt (shrK A) (Nonce NB)) \<in> set evs"
+by (blast dest!: NB_Crypt_imp_Server_msg)
+
+
+(*B only issues challenges in response to WL1.  Not used.*)
+lemma B_said_WL2:
+     "[| Says B A (Nonce NB) \<in> set evs;  B \<noteq> Spy;  evs \<in> woolam |]
+      ==> \<exists>A'. Says A' B (Agent A) \<in> set evs"
+apply (erule rev_mp, erule woolam.induct, force, simp_all)
+apply blast+
+done
+
+
+(**CANNOT be proved because A doesn't know where challenges come from...*)
+lemma "[| A \<notin> bad;  B \<noteq> Spy;  evs \<in> woolam |]
+  ==> Crypt (shrK A) (Nonce NB) \<in> parts (spies evs) &
+      Says B A (Nonce NB) \<in> set evs
+      --> Says A B (Crypt (shrK A) (Nonce NB)) \<in> set evs"
+apply (erule rev_mp, erule woolam.induct, force, simp_all)
+apply blast
+apply auto
+oops
 
 end
