src/HOL/Auth/Yahalom.thy
@@ -8,73 +8,633 @@ Inductive relation "yahalom" for the Yahalom protocol.
 From page 257 of
   Burrows, Abadi and Needham.  A Logic of Authentication.
   Proc. Royal Soc. 426 (1989)
+
+This theory has the prototypical example of a secrecy relation, KeyCryptNonce.
 *)
 
-Yahalom = Shared + 
+theory Yahalom = Shared:
 
-consts  yahalom   :: event list set
+consts  yahalom   :: "event list set"
 inductive "yahalom"
-  intrs 
+  intros 
          (*Initial trace is empty*)
-    Nil  "[] \\<in> yahalom"
+   Nil:  "[] \<in> yahalom"
 
          (*The spy MAY say anything he CAN say.  We do not expect him to
            invent new nonces here, but he can also use NS1.  Common to
            all similar protocols.*)
-    Fake "[| evsf \\<in> yahalom;  X \\<in> synth (analz (knows Spy evsf)) |]
-          ==> Says Spy B X  # evsf \\<in> yahalom"
+   Fake: "[| evsf \<in> yahalom;  X \<in> synth (analz (knows Spy evsf)) |]
+          ==> Says Spy B X  # evsf \<in> yahalom"
 
          (*A message that has been sent can be received by the
            intended recipient.*)
-    Reception "[| evsr \\<in> yahalom;  Says A B X \\<in> set evsr |]
-               ==> Gets B X # evsr \\<in> yahalom"
+   Reception: "[| evsr \<in> yahalom;  Says A B X \<in> set evsr |]
+               ==> Gets B X # evsr \<in> yahalom"
 
          (*Alice initiates a protocol run*)
-    YM1  "[| evs1 \\<in> yahalom;  Nonce NA \\<notin> used evs1 |]
-          ==> Says A B {|Agent A, Nonce NA|} # evs1 \\<in> yahalom"
+   YM1:  "[| evs1 \<in> yahalom;  Nonce NA \<notin> used evs1 |]
+          ==> Says A B {|Agent A, Nonce NA|} # evs1 \<in> yahalom"
 
          (*Bob's response to Alice's message.*)
-    YM2  "[| evs2 \\<in> yahalom;  Nonce NB \\<notin> used evs2;
-             Gets B {|Agent A, Nonce NA|} \\<in> set evs2 |]
+   YM2:  "[| evs2 \<in> yahalom;  Nonce NB \<notin> used evs2;
+             Gets B {|Agent A, Nonce NA|} \<in> set evs2 |]
           ==> Says B Server 
                   {|Agent B, Crypt (shrK B) {|Agent A, Nonce NA, Nonce NB|}|}
-                # evs2 \\<in> yahalom"
+                # evs2 \<in> yahalom"
 
          (*The Server receives Bob's message.  He responds by sending a
             new session key to Alice, with a packet for forwarding to Bob.*)
-    YM3  "[| evs3 \\<in> yahalom;  Key KAB \\<notin> used evs3;
+   YM3:  "[| evs3 \<in> yahalom;  Key KAB \<notin> used evs3;
              Gets Server 
                   {|Agent B, Crypt (shrK B) {|Agent A, Nonce NA, Nonce NB|}|}
-               \\<in> set evs3 |]
+               \<in> set evs3 |]
           ==> Says Server A
                    {|Crypt (shrK A) {|Agent B, Key KAB, Nonce NA, Nonce NB|},
                      Crypt (shrK B) {|Agent A, Key KAB|}|}
-                # evs3 \\<in> yahalom"
+                # evs3 \<in> yahalom"
 
          (*Alice receives the Server's (?) message, checks her Nonce, and
            uses the new session key to send Bob his Nonce.  The premise
-           A \\<noteq> Server is needed to prove Says_Server_not_range.*)
-    YM4  "[| evs4 \\<in> yahalom;  A \\<noteq> Server;
+           A \<noteq> Server is needed to prove Says_Server_not_range.*)
+   YM4:  "[| evs4 \<in> yahalom;  A \<noteq> Server;
              Gets A {|Crypt(shrK A) {|Agent B, Key K, Nonce NA, Nonce NB|}, X|}
-                \\<in> set evs4;
-             Says A B {|Agent A, Nonce NA|} \\<in> set evs4 |]
-          ==> Says A B {|X, Crypt K (Nonce NB)|} # evs4 \\<in> yahalom"
+                \<in> set evs4;
+             Says A B {|Agent A, Nonce NA|} \<in> set evs4 |]
+          ==> Says A B {|X, Crypt K (Nonce NB)|} # evs4 \<in> yahalom"
 
          (*This message models possible leaks of session keys.  The Nonces
            identify the protocol run.  Quoting Server here ensures they are
            correct.*)
-    Oops "[| evso \\<in> yahalom;  
+   Oops: "[| evso \<in> yahalom;  
              Says Server A {|Crypt (shrK A)
                                    {|Agent B, Key K, Nonce NA, Nonce NB|},
-                             X|}  \\<in> set evso |]
-          ==> Notes Spy {|Nonce NA, Nonce NB, Key K|} # evso \\<in> yahalom"
+                             X|}  \<in> set evso |]
+          ==> Notes Spy {|Nonce NA, Nonce NB, Key K|} # evso \<in> yahalom"
 
 
 constdefs 
-  KeyWithNonce :: [key, nat, event list] => bool
+  KeyWithNonce :: "[key, nat, event list] => bool"
   "KeyWithNonce K NB evs ==
-     \\<exists>A B na X. 
+     \<exists>A B na X. 
        Says Server A {|Crypt (shrK A) {|Agent B, Key K, na, Nonce NB|}, X|} 
-         \\<in> set evs"
+         \<in> set evs"
+
+
+declare Says_imp_knows_Spy [THEN analz.Inj, dest]
+declare parts.Body  [dest]
+declare Fake_parts_insert_in_Un  [dest]
+declare analz_into_parts [dest]
+
+(*A "possibility property": there are traces that reach the end*)
+lemma "A \<noteq> Server  
+      ==> \<exists>X NB K. \<exists>evs \<in> yahalom.           
+             Says A B {|X, Crypt K (Nonce NB)|} \<in> set evs"
+apply (intro exI bexI)
+apply (rule_tac [2] yahalom.Nil
+                    [THEN yahalom.YM1, THEN yahalom.Reception, 
+                     THEN yahalom.YM2, THEN yahalom.Reception, 
+                     THEN yahalom.YM3, THEN yahalom.Reception, 
+                     THEN yahalom.YM4])
+apply possibility
+done
+
+lemma Gets_imp_Says:
+     "[| Gets B X \<in> set evs; evs \<in> yahalom |] ==> \<exists>A. Says A B X \<in> set evs"
+by (erule rev_mp, erule yahalom.induct, auto)
+
+(*Must be proved separately for each protocol*)
+lemma Gets_imp_knows_Spy:
+     "[| Gets B X \<in> set evs; evs \<in> yahalom |]  ==> X \<in> knows Spy evs"
+by (blast dest!: Gets_imp_Says Says_imp_knows_Spy)
+
+declare Gets_imp_knows_Spy [THEN analz.Inj, dest]
+
+
+(**** Inductive proofs about yahalom ****)
+
+(*Lets us treat YM4 using a similar argument as for the Fake case.*)
+lemma YM4_analz_knows_Spy:
+     "[| Gets A {|Crypt (shrK A) Y, X|} \<in> set evs;  evs \<in> yahalom |]   
+      ==> X \<in> analz (knows Spy evs)"
+by blast
+
+lemmas YM4_parts_knows_Spy = 
+       YM4_analz_knows_Spy [THEN analz_into_parts, standard]
+
+(*For Oops*)
+lemma YM4_Key_parts_knows_Spy:
+     "Says Server A {|Crypt (shrK A) {|B,K,NA,NB|}, X|} \<in> set evs  
+      ==> K \<in> parts (knows Spy evs)"
+by (blast dest!: parts.Body Says_imp_knows_Spy [THEN parts.Inj])
+
+
+(** Theorems of the form X \<notin> parts (knows Spy evs) imply that NOBODY
+    sends messages containing X! **)
+
+(*Spy never sees a good agent's shared key!*)
+lemma Spy_see_shrK [simp]:
+     "evs \<in> yahalom ==> (Key (shrK A) \<in> parts (knows Spy evs)) = (A \<in> bad)"
+apply (erule yahalom.induct, force, 
+       drule_tac [6] YM4_parts_knows_Spy, simp_all)
+apply blast+
+done
+
+lemma Spy_analz_shrK [simp]:
+     "evs \<in> yahalom ==> (Key (shrK A) \<in> analz (knows Spy evs)) = (A \<in> bad)"
+by auto
+
+lemma Spy_see_shrK_D [dest!]:
+     "[|Key (shrK A) \<in> parts (knows Spy evs);  evs \<in> yahalom|] ==> A \<in> bad"
+by (blast dest: Spy_see_shrK)
+
+(*Nobody can have used non-existent keys!  Needed to apply analz_insert_Key*)
+lemma new_keys_not_used [rule_format, simp]:
+ "evs \<in> yahalom ==> Key K \<notin> used evs --> K \<notin> keysFor (parts (knows Spy evs))"
+apply (erule yahalom.induct, force, 
+       frule_tac [6] YM4_parts_knows_Spy, simp_all)
+(*Fake, YM3, YM4*)
+apply (blast dest!: keysFor_parts_insert)+
+done
+
+
+(*Earlier, all protocol proofs declared this theorem.  
+  But only a few proofs need it, e.g. Yahalom and Kerberos IV.*)
+lemma new_keys_not_analzd:
+ "[|evs \<in> yahalom; Key K \<notin> used evs|] ==> K \<notin> keysFor (analz (knows Spy evs))"
+by (blast dest: new_keys_not_used intro: keysFor_mono [THEN subsetD]) 
+
+
+(*Describes the form of K when the Server sends this message.  Useful for
+  Oops as well as main secrecy property.*)
+lemma Says_Server_not_range [simp]:
+     "[| Says Server A {|Crypt (shrK A) {|Agent B, Key K, na, nb|}, X|}  
+           \<in> set evs;   evs \<in> yahalom |]                                 
+      ==> K \<notin> range shrK"
+apply (erule rev_mp, erule yahalom.induct, simp_all)
+apply blast
+done
+
+
+(*For proofs involving analz.
+val analz_knows_Spy_tac = 
+    ftac YM4_analz_knows_Spy 7 THEN assume_tac 7
+*)
+
+(****
+ The following is to prove theorems of the form
+
+  Key K \<in> analz (insert (Key KAB) (knows Spy evs)) ==>
+  Key K \<in> analz (knows Spy evs)
+
+ A more general formula must be proved inductively.
+****)
+
+(** Session keys are not used to encrypt other session keys **)
+
+lemma analz_image_freshK [rule_format]:
+ "evs \<in> yahalom ==>                                
+   \<forall>K KK. KK <= - (range shrK) -->                  
+          (Key K \<in> analz (Key`KK Un (knows Spy evs))) =   
+          (K \<in> KK | Key K \<in> analz (knows Spy evs))"
+apply (erule yahalom.induct, force, 
+       drule_tac [6] YM4_analz_knows_Spy)
+apply analz_freshK
+apply spy_analz
+apply (simp only: Says_Server_not_range analz_image_freshK_simps)
+done
+
+lemma analz_insert_freshK:
+     "[| evs \<in> yahalom;  KAB \<notin> range shrK |] ==>      
+      Key K \<in> analz (insert (Key KAB) (knows Spy evs)) =   
+      (K = KAB | Key K \<in> analz (knows Spy evs))"
+by (simp only: analz_image_freshK analz_image_freshK_simps)
+
+
+(*** The Key K uniquely identifies the Server's  message. **)
+
+lemma unique_session_keys:
+     "[| Says Server A                                                  
+          {|Crypt (shrK A) {|Agent B, Key K, na, nb|}, X|} \<in> set evs;  
+        Says Server A'                                                 
+          {|Crypt (shrK A') {|Agent B', Key K, na', nb'|}, X'|} \<in> set evs;  
+        evs \<in> yahalom |]                                     
+     ==> A=A' & B=B' & na=na' & nb=nb'"
+apply (erule rev_mp, erule rev_mp)
+apply (erule yahalom.induct, simp_all)
+(*YM3, by freshness, and YM4*)
+apply blast+
+done
+
+
+(** Crucial secrecy property: Spy does not see the keys sent in msg YM3 **)
+
+lemma secrecy_lemma:
+     "[| A \<notin> bad;  B \<notin> bad;  evs \<in> yahalom |]                 
+      ==> Says Server A                                         
+            {|Crypt (shrK A) {|Agent B, Key K, na, nb|},        
+              Crypt (shrK B) {|Agent A, Key K|}|}               
+           \<in> set evs -->                                        
+          Notes Spy {|na, nb, Key K|} \<notin> set evs -->            
+          Key K \<notin> analz (knows Spy evs)"
+apply (erule yahalom.induct, force, 
+       drule_tac [6] YM4_analz_knows_Spy)
+apply (simp_all add: pushes analz_insert_eq analz_insert_freshK)
+apply spy_analz  (*Fake*)
+apply (blast dest: unique_session_keys)+  (*YM3, Oops*)
+done
+
+(*Final version*)
+lemma Spy_not_see_encrypted_key:
+     "[| Says Server A                                          
+            {|Crypt (shrK A) {|Agent B, Key K, na, nb|},        
+              Crypt (shrK B) {|Agent A, Key K|}|}               
+           \<in> set evs;                                           
+         Notes Spy {|na, nb, Key K|} \<notin> set evs;                
+         A \<notin> bad;  B \<notin> bad;  evs \<in> yahalom |]                 
+      ==> Key K \<notin> analz (knows Spy evs)"
+by (blast dest: secrecy_lemma)
+
+
+(** Security Guarantee for A upon receiving YM3 **)
+
+(*If the encrypted message appears then it originated with the Server*)
+lemma A_trusts_YM3:
+     "[| Crypt (shrK A) {|Agent B, Key K, na, nb|} \<in> parts (knows Spy evs);  
+         A \<notin> bad;  evs \<in> yahalom |]                           
+       ==> Says Server A                                             
+            {|Crypt (shrK A) {|Agent B, Key K, na, nb|},             
+              Crypt (shrK B) {|Agent A, Key K|}|}                    
+           \<in> set evs"
+apply (erule rev_mp)
+apply (erule yahalom.induct, force, 
+       frule_tac [6] YM4_parts_knows_Spy, simp_all)
+(*Fake, YM3*)
+apply blast+
+done
+
+(*The obvious combination of A_trusts_YM3 with Spy_not_see_encrypted_key*)
+lemma A_gets_good_key:
+     "[| Crypt (shrK A) {|Agent B, Key K, na, nb|} \<in> parts (knows Spy evs);  
+         Notes Spy {|na, nb, Key K|} \<notin> set evs;                
+         A \<notin> bad;  B \<notin> bad;  evs \<in> yahalom |]                 
+      ==> Key K \<notin> analz (knows Spy evs)"
+by (blast dest!: A_trusts_YM3 Spy_not_see_encrypted_key)
+
+(** Security Guarantees for B upon receiving YM4 **)
+
+(*B knows, by the first part of A's message, that the Server distributed 
+  the key for A and B.  But this part says nothing about nonces.*)
+lemma B_trusts_YM4_shrK:
+     "[| Crypt (shrK B) {|Agent A, Key K|} \<in> parts (knows Spy evs);       
+         B \<notin> bad;  evs \<in> yahalom |]                                  
+      ==> \<exists>NA NB. Says Server A                                     
+                      {|Crypt (shrK A) {|Agent B, Key K,              
+                                         Nonce NA, Nonce NB|},        
+                        Crypt (shrK B) {|Agent A, Key K|}|}           
+                     \<in> set evs"
+apply (erule rev_mp)
+apply (erule yahalom.induct, force, 
+       frule_tac [6] YM4_parts_knows_Spy, simp_all)
+(*Fake, YM3*)
+apply blast+
+done
+
+(*B knows, by the second part of A's message, that the Server distributed 
+  the key quoting nonce NB.  This part says nothing about agent names. 
+  Secrecy of NB is crucial.  Note that  Nonce NB \<notin> analz(knows Spy evs)  must
+  be the FIRST antecedent of the induction formula.*)
+lemma B_trusts_YM4_newK[rule_format]:
+     "[|Crypt K (Nonce NB) \<in> parts (knows Spy evs);
+        Nonce NB \<notin> analz (knows Spy evs);  evs \<in> yahalom|]
+      ==> \<exists>A B NA. Says Server A                           
+                      {|Crypt (shrK A) {|Agent B, Key K, Nonce NA, Nonce NB|},
+                        Crypt (shrK B) {|Agent A, Key K|}|}   
+                     \<in> set evs"
+apply (erule rev_mp, erule rev_mp)
+apply (erule yahalom.induct, force, 
+       frule_tac [6] YM4_parts_knows_Spy)
+apply (analz_mono_contra, simp_all)
+(*Fake, YM3*)
+apply blast
+apply blast
+(*YM4*)
+(*A is uncompromised because NB is secure
+  A's certificate guarantees the existence of the Server message*)
+apply (blast dest!: Gets_imp_Says Crypt_Spy_analz_bad 
+             dest: Says_imp_spies 
+                   parts.Inj [THEN parts.Fst, THEN A_trusts_YM3])
+done
+
+
+(**** Towards proving secrecy of Nonce NB ****)
+
+(** Lemmas about the predicate KeyWithNonce **)
+
+lemma KeyWithNonceI: 
+ "Says Server A                                               
+          {|Crypt (shrK A) {|Agent B, Key K, na, Nonce NB|}, X|}  
+        \<in> set evs ==> KeyWithNonce K NB evs"
+by (unfold KeyWithNonce_def, blast)
+
+lemma KeyWithNonce_Says [simp]: 
+   "KeyWithNonce K NB (Says S A X # evs) =                                     
+      (Server = S &
+       (\<exists>B n X'. X = {|Crypt (shrK A) {|Agent B, Key K, n, Nonce NB|}, X'|})  
+      | KeyWithNonce K NB evs)"
+by (simp add: KeyWithNonce_def, blast)
+
+
+lemma KeyWithNonce_Notes [simp]: 
+   "KeyWithNonce K NB (Notes A X # evs) = KeyWithNonce K NB evs"
+by (simp add: KeyWithNonce_def)
+
+lemma KeyWithNonce_Gets [simp]: 
+   "KeyWithNonce K NB (Gets A X # evs) = KeyWithNonce K NB evs"
+by (simp add: KeyWithNonce_def)
+
+(*A fresh key cannot be associated with any nonce 
+  (with respect to a given trace). *)
+lemma fresh_not_KeyWithNonce: 
+ "Key K \<notin> used evs ==> ~ KeyWithNonce K NB evs"
+by (unfold KeyWithNonce_def, blast)
+
+(*The Server message associates K with NB' and therefore not with any 
+  other nonce NB.*)
+lemma Says_Server_KeyWithNonce: 
+ "[| Says Server A {|Crypt (shrK A) {|Agent B, Key K, na, Nonce NB'|}, X|}  
+       \<in> set evs;                                                  
+     NB \<noteq> NB';  evs \<in> yahalom |]                                  
+  ==> ~ KeyWithNonce K NB evs"
+by (unfold KeyWithNonce_def, blast dest: unique_session_keys)
+
+
+(*The only nonces that can be found with the help of session keys are
+  those distributed as nonce NB by the Server.  The form of the theorem
+  recalls analz_image_freshK, but it is much more complicated.*)
+
+
+(*As with analz_image_freshK, we take some pains to express the property
+  as a logical equivalence so that the simplifier can apply it.*)
+lemma Nonce_secrecy_lemma:
+     "P --> (X \<in> analz (G Un H)) --> (X \<in> analz H)  ==>  
+      P --> (X \<in> analz (G Un H)) = (X \<in> analz H)"
+by (blast intro: analz_mono [THEN subsetD])
+
+lemma Nonce_secrecy:
+     "evs \<in> yahalom ==>                                       
+      (\<forall>KK. KK <= - (range shrK) -->                       
+           (\<forall>K \<in> KK. ~ KeyWithNonce K NB evs)   -->         
+           (Nonce NB \<in> analz (Key`KK Un (knows Spy evs))) =      
+           (Nonce NB \<in> analz (knows Spy evs)))"
+apply (erule yahalom.induct, force, 
+       frule_tac [6] YM4_analz_knows_Spy)
+apply (safe del: allI impI intro!: Nonce_secrecy_lemma [THEN impI, THEN allI])
+apply (simp_all del: image_insert image_Un 
+       add: analz_image_freshK_simps split_ifs
+            all_conj_distrib ball_conj_distrib 
+            analz_image_freshK fresh_not_KeyWithNonce
+            imp_disj_not1               (*Moves NBa\<noteq>NB to the front*)
+            Says_Server_KeyWithNonce)
+(*For Oops, simplification proves NBa\<noteq>NB.  By Says_Server_KeyWithNonce,
+  we get (~ KeyWithNonce K NB evs); then simplification can apply the
+  induction hypothesis with KK = {K}.*)
+(*Fake*) 
+apply spy_analz
+(*YM4*)  (** LEVEL 6 **)
+apply (erule_tac V = "\<forall>KK. ?P KK" in thin_rl)
+apply clarify
+(*If A \<in> bad then NBa is known, therefore NBa \<noteq> NB.  Previous two steps make
+  the next step faster.*)
+apply (blast dest!: Gets_imp_Says Says_imp_spies Crypt_Spy_analz_bad
+         dest: analz.Inj
+           parts.Inj [THEN parts.Fst, THEN A_trusts_YM3, THEN KeyWithNonceI])
+done
+
+
+(*Version required below: if NB can be decrypted using a session key then it
+  was distributed with that key.  The more general form above is required
+  for the induction to carry through.*)
+lemma single_Nonce_secrecy:
+     "[| Says Server A                                                
+          {|Crypt (shrK A) {|Agent B, Key KAB, na, Nonce NB'|}, X|}   
+         \<in> set evs;                                                   
+         NB \<noteq> NB';  KAB \<notin> range shrK;  evs \<in> yahalom |]             
+      ==> (Nonce NB \<in> analz (insert (Key KAB) (knows Spy evs))) =         
+          (Nonce NB \<in> analz (knows Spy evs))"
+by (simp_all del: image_insert image_Un imp_disjL
+             add: analz_image_freshK_simps split_ifs
+                  Nonce_secrecy Says_Server_KeyWithNonce);
+
+
+(*** The Nonce NB uniquely identifies B's message. ***)
+
+lemma unique_NB:
+     "[| Crypt (shrK B) {|Agent A, Nonce NA, nb|} \<in> parts (knows Spy evs);     
+         Crypt (shrK B') {|Agent A', Nonce NA', nb|} \<in> parts (knows Spy evs);  
+        evs \<in> yahalom;  B \<notin> bad;  B' \<notin> bad |]   
+      ==> NA' = NA & A' = A & B' = B"
+apply (erule rev_mp, erule rev_mp)
+apply (erule yahalom.induct, force, 
+       frule_tac [6] YM4_parts_knows_Spy, simp_all)
+(*Fake, and YM2 by freshness*)
+apply blast+
+done
+
+
+(*Variant useful for proving secrecy of NB.  Because nb is assumed to be 
+  secret, we no longer must assume B, B' not bad.*)
+lemma Says_unique_NB:
+     "[| Says C S   {|X,  Crypt (shrK B) {|Agent A, Nonce NA, nb|}|}     
+           \<in> set evs;                           
+         Gets S' {|X', Crypt (shrK B') {|Agent A', Nonce NA', nb|}|}     
+           \<in> set evs;                                                    
+         nb \<notin> analz (knows Spy evs);  evs \<in> yahalom |]                  
+      ==> NA' = NA & A' = A & B' = B"
+by (blast dest!: Gets_imp_Says Crypt_Spy_analz_bad 
+          dest: Says_imp_spies unique_NB parts.Inj analz.Inj)
+
+
+(** A nonce value is never used both as NA and as NB **)
+
+lemma no_nonce_YM1_YM2:
+     "[|Crypt (shrK B') {|Agent A', Nonce NB, nb'|} \<in> parts(knows Spy evs);
+        Nonce NB \<notin> analz (knows Spy evs);  evs \<in> yahalom|]
+  ==> Crypt (shrK B)  {|Agent A, na, Nonce NB|} \<notin> parts(knows Spy evs)"
+apply (erule rev_mp, erule rev_mp)
+apply (erule yahalom.induct, force, 
+       frule_tac [6] YM4_parts_knows_Spy)
+apply (analz_mono_contra, simp_all)
+(*Fake, YM2*)
+apply blast+
+done
+
+(*The Server sends YM3 only in response to YM2.*)
+lemma Says_Server_imp_YM2:
+     "[| Says Server A {|Crypt (shrK A) {|Agent B, k, na, nb|}, X|} \<in> set evs;
+         evs \<in> yahalom |]                                              
+      ==> Gets Server {| Agent B, Crypt (shrK B) {|Agent A, na, nb|} |}  
+             \<in> set evs"
+apply (erule rev_mp, erule yahalom.induct)
+apply auto
+done
+
+
+(*A vital theorem for B, that nonce NB remains secure from the Spy.*)
+lemma Spy_not_see_NB :
+     "[| Says B Server                                                     
+	        {|Agent B, Crypt (shrK B) {|Agent A, Nonce NA, Nonce NB|}|}  
+	   \<in> set evs;
+	 (\<forall>k. Notes Spy {|Nonce NA, Nonce NB, k|} \<notin> set evs);
+         A \<notin> bad;  B \<notin> bad;  evs \<in> yahalom |]   
+      ==> Nonce NB \<notin> analz (knows Spy evs)"
+apply (erule rev_mp, erule rev_mp)
+apply (erule yahalom.induct, force, 
+       frule_tac [6] YM4_analz_knows_Spy)
+apply (simp_all add: split_ifs pushes new_keys_not_analzd analz_insert_eq
+                     analz_insert_freshK)
+(*Fake*)
+apply spy_analz
+(*YM1: NB=NA is impossible anyway, but NA is secret because it is fresh!*)
+apply blast
+(*YM2*)
+apply blast
+(*Prove YM3 by showing that no NB can also be an NA*)
+apply (blast dest!: no_nonce_YM1_YM2 dest: Gets_imp_Says Says_unique_NB)
+(** LEVEL 7: YM4 and Oops remain **)
+apply (clarify, simp add: all_conj_distrib)
+(*YM4: key K is visible to Spy, contradicting session key secrecy theorem*) 
+(*Case analysis on Aa:bad; PROOF FAILED problems
+  use Says_unique_NB to identify message components: Aa=A, Ba=B*)  
+apply (blast dest!: Says_unique_NB 
+                    parts.Inj [THEN parts.Fst, THEN A_trusts_YM3] 
+             dest: Gets_imp_Says Says_imp_spies Says_Server_imp_YM2
+                   Spy_not_see_encrypted_key)
+(*Oops case: if the nonce is betrayed now, show that the Oops event is 
+  covered by the quantified Oops assumption.*)
+apply (clarify, simp add: all_conj_distrib)
+apply (frule Says_Server_imp_YM2, assumption)
+apply (case_tac "NB = NBa")
+(*If NB=NBa then all other components of the Oops message agree*)
+apply (blast dest: Says_unique_NB)
+(*case NB \<noteq> NBa*)
+apply (simp add: single_Nonce_secrecy)
+apply (blast dest!: no_nonce_YM1_YM2 (*to prove NB\<noteq>NAa*))
+done
+
+
+(*B's session key guarantee from YM4.  The two certificates contribute to a
+  single conclusion about the Server's message.  Note that the "Notes Spy"
+  assumption must quantify over \<forall>POSSIBLE keys instead of our particular K.
+  If this run is broken and the spy substitutes a certificate containing an
+  old key, B has no means of telling.*)
+lemma B_trusts_YM4:
+     "[| Gets B {|Crypt (shrK B) {|Agent A, Key K|},                   
+                  Crypt K (Nonce NB)|} \<in> set evs;                      
+         Says B Server                                                    
+           {|Agent B, Crypt (shrK B) {|Agent A, Nonce NA, Nonce NB|}|}    
+           \<in> set evs;                                                     
+         \<forall>k. Notes Spy {|Nonce NA, Nonce NB, k|} \<notin> set evs;           
+         A \<notin> bad;  B \<notin> bad;  evs \<in> yahalom |]        
+       ==> Says Server A                                                  
+                   {|Crypt (shrK A) {|Agent B, Key K,                     
+                             Nonce NA, Nonce NB|},                        
+                     Crypt (shrK B) {|Agent A, Key K|}|}                  
+             \<in> set evs"
+by (blast dest: Spy_not_see_NB Says_unique_NB 
+                Says_Server_imp_YM2 B_trusts_YM4_newK)
+
+
+
+(*The obvious combination of B_trusts_YM4 with Spy_not_see_encrypted_key*)
+lemma B_gets_good_key:
+     "[| Gets B {|Crypt (shrK B) {|Agent A, Key K|},
+                  Crypt K (Nonce NB)|} \<in> set evs;
+         Says B Server                                                    
+           {|Agent B, Crypt (shrK B) {|Agent A, Nonce NA, Nonce NB|}|}    
+           \<in> set evs;                                                     
+         \<forall>k. Notes Spy {|Nonce NA, Nonce NB, k|} \<notin> set evs;           
+         A \<notin> bad;  B \<notin> bad;  evs \<in> yahalom |]                 
+      ==> Key K \<notin> analz (knows Spy evs)"
+by (blast dest!: B_trusts_YM4 Spy_not_see_encrypted_key)
+
+
+(*** Authenticating B to A ***)
+
+(*The encryption in message YM2 tells us it cannot be faked.*)
+lemma B_Said_YM2 [rule_format]:
+     "[|Crypt (shrK B) {|Agent A, Nonce NA, nb|} \<in> parts (knows Spy evs);
+        evs \<in> yahalom|]
+      ==> B \<notin> bad -->
+          Says B Server {|Agent B, Crypt (shrK B) {|Agent A, Nonce NA, nb|}|}
+            \<in> set evs"
+apply (erule rev_mp, erule yahalom.induct, force, 
+       frule_tac [6] YM4_parts_knows_Spy, simp_all)
+(*Fake*)
+apply blast
+done
+
+(*If the server sends YM3 then B sent YM2*)
+lemma YM3_auth_B_to_A_lemma:
+     "[|Says Server A {|Crypt (shrK A) {|Agent B, Key K, Nonce NA, nb|}, X|}  
+       \<in> set evs;  evs \<in> yahalom|]
+      ==> B \<notin> bad -->                                                         
+          Says B Server {|Agent B, Crypt (shrK B) {|Agent A, Nonce NA, nb|}|}
+            \<in> set evs"
+apply (erule rev_mp, erule yahalom.induct, simp_all)
+(*YM3, YM4*)
+apply (blast dest!: B_Said_YM2)+
+done
+
+(*If A receives YM3 then B has used nonce NA (and therefore is alive)*)
+lemma YM3_auth_B_to_A:
+     "[| Gets A {|Crypt (shrK A) {|Agent B, Key K, Nonce NA, nb|}, X|}  
+           \<in> set evs;                                                     
+         A \<notin> bad;  B \<notin> bad;  evs \<in> yahalom |]                         
+      ==> Says B Server {|Agent B, Crypt (shrK B) {|Agent A, Nonce NA, nb|}|}  
+       \<in> set evs"
+by (blast dest!: A_trusts_YM3 YM3_auth_B_to_A_lemma elim: knows_Spy_partsEs)
+
+
+(*** Authenticating A to B using the certificate Crypt K (Nonce NB) ***)
+
+(*Assuming the session key is secure, if both certificates are present then
+  A has said NB.  We can't be sure about the rest of A's message, but only
+  NB matters for freshness.*)  
+lemma A_Said_YM3_lemma [rule_format]:
+     "evs \<in> yahalom
+      ==> Key K \<notin> analz (knows Spy evs) -->
+          Crypt K (Nonce NB) \<in> parts (knows Spy evs) -->
+          Crypt (shrK B) {|Agent A, Key K|} \<in> parts (knows Spy evs) -->
+          B \<notin> bad -->
+          (\<exists>X. Says A B {|X, Crypt K (Nonce NB)|} \<in> set evs)"
+apply (erule yahalom.induct, force, 
+       frule_tac [6] YM4_parts_knows_Spy)
+apply (analz_mono_contra, simp_all)
+(*Fake*)
+apply blast
+(*YM3: by new_keys_not_used we note that Crypt K (Nonce NB) could not exist*)
+apply (force dest!: Crypt_imp_keysFor)
+(*YM4: was Crypt K (Nonce NB) the very last message?  If not, use ind. hyp.*)
+apply (simp add: ex_disj_distrib)
+(*yes: apply unicity of session keys*)
+apply (blast dest!: Gets_imp_Says A_trusts_YM3 B_trusts_YM4_shrK
+                    Crypt_Spy_analz_bad 
+             dest: Says_imp_knows_Spy [THEN parts.Inj] unique_session_keys)
+done
+
+(*If B receives YM4 then A has used nonce NB (and therefore is alive).
+  Moreover, A associates K with NB (thus is talking about the same run).
+  Other premises guarantee secrecy of K.*)
+lemma YM4_imp_A_Said_YM3 [rule_format]:
+     "[| Gets B {|Crypt (shrK B) {|Agent A, Key K|},
+                  Crypt K (Nonce NB)|} \<in> set evs;
+         Says B Server
+           {|Agent B, Crypt (shrK B) {|Agent A, Nonce NA, Nonce NB|}|}
+           \<in> set evs;
+         (\<forall>NA k. Notes Spy {|Nonce NA, Nonce NB, k|} \<notin> set evs);
+         A \<notin> bad;  B \<notin> bad;  evs \<in> yahalom |]
+      ==> \<exists>X. Says A B {|X, Crypt K (Nonce NB)|} \<in> set evs"
+by (blast intro!: A_Said_YM3_lemma 
+          dest: Spy_not_see_encrypted_key B_trusts_YM4 Gets_imp_Says)
 
 end
