src/HOL/Auth/Yahalom2.thy
@@ -13,64 +13,389 @@ From page 259 of
   Proc. Royal Soc. 426 (1989)
 *)
 
-Yahalom2 = Shared + 
+theory Yahalom2 = Shared:
 
-consts  yahalom   :: event list set
+consts  yahalom   :: "event list set"
 inductive "yahalom"
-  intrs 
+  intros
          (*Initial trace is empty*)
-    Nil  "[] \\<in> yahalom"
+   Nil:  "[] \<in> yahalom"
 
          (*The spy MAY say anything he CAN say.  We do not expect him to
            invent new nonces here, but he can also use NS1.  Common to
            all similar protocols.*)
-    Fake "[| evsf \\<in> yahalom;  X \\<in> synth (analz (knows Spy evsf)) |]
-          ==> Says Spy B X  # evsf \\<in> yahalom"
+   Fake: "[| evsf \<in> yahalom;  X \<in> synth (analz (knows Spy evsf)) |]
+          ==> Says Spy B X  # evsf \<in> yahalom"
 
          (*A message that has been sent can be received by the
            intended recipient.*)
-    Reception "[| evsr \\<in> yahalom;  Says A B X \\<in> set evsr |]
-               ==> Gets B X # evsr \\<in> yahalom"
+   Reception: "[| evsr \<in> yahalom;  Says A B X \<in> set evsr |]
+               ==> Gets B X # evsr \<in> yahalom"
 
          (*Alice initiates a protocol run*)
-    YM1  "[| evs1 \\<in> yahalom;  Nonce NA \\<notin> used evs1 |]
-          ==> Says A B {|Agent A, Nonce NA|} # evs1 \\<in> yahalom"
+   YM1:  "[| evs1 \<in> yahalom;  Nonce NA \<notin> used evs1 |]
+          ==> Says A B {|Agent A, Nonce NA|} # evs1 \<in> yahalom"
 
          (*Bob's response to Alice's message.*)
-    YM2  "[| evs2 \\<in> yahalom;  Nonce NB \\<notin> used evs2;
-             Gets B {|Agent A, Nonce NA|} \\<in> set evs2 |]
-          ==> Says B Server 
+   YM2:  "[| evs2 \<in> yahalom;  Nonce NB \<notin> used evs2;
+             Gets B {|Agent A, Nonce NA|} \<in> set evs2 |]
+          ==> Says B Server
                   {|Agent B, Nonce NB, Crypt (shrK B) {|Agent A, Nonce NA|}|}
-                # evs2 \\<in> yahalom"
+                # evs2 \<in> yahalom"
 
          (*The Server receives Bob's message.  He responds by sending a
            new session key to Alice, with a certificate for forwarding to Bob.
            Both agents are quoted in the 2nd certificate to prevent attacks!*)
-    YM3  "[| evs3 \\<in> yahalom;  Key KAB \\<notin> used evs3;
+   YM3:  "[| evs3 \<in> yahalom;  Key KAB \<notin> used evs3;
              Gets Server {|Agent B, Nonce NB,
 			   Crypt (shrK B) {|Agent A, Nonce NA|}|}
-               \\<in> set evs3 |]
+               \<in> set evs3 |]
           ==> Says Server A
-               {|Nonce NB, 
+               {|Nonce NB,
                  Crypt (shrK A) {|Agent B, Key KAB, Nonce NA|},
                  Crypt (shrK B) {|Agent A, Agent B, Key KAB, Nonce NB|}|}
-                 # evs3 \\<in> yahalom"
+                 # evs3 \<in> yahalom"
 
          (*Alice receives the Server's (?) message, checks her Nonce, and
            uses the new session key to send Bob his Nonce.*)
-    YM4  "[| evs4 \\<in> yahalom;  
+   YM4:  "[| evs4 \<in> yahalom;
              Gets A {|Nonce NB, Crypt (shrK A) {|Agent B, Key K, Nonce NA|},
-                      X|}  \\<in> set evs4;
-             Says A B {|Agent A, Nonce NA|} \\<in> set evs4 |]
-          ==> Says A B {|X, Crypt K (Nonce NB)|} # evs4 \\<in> yahalom"
+                      X|}  \<in> set evs4;
+             Says A B {|Agent A, Nonce NA|} \<in> set evs4 |]
+          ==> Says A B {|X, Crypt K (Nonce NB)|} # evs4 \<in> yahalom"
 
          (*This message models possible leaks of session keys.  The nonces
            identify the protocol run.  Quoting Server here ensures they are
            correct. *)
-    Oops "[| evso \\<in> yahalom;  
-             Says Server A {|Nonce NB, 
+   Oops: "[| evso \<in> yahalom;
+             Says Server A {|Nonce NB,
                              Crypt (shrK A) {|Agent B, Key K, Nonce NA|},
-                             X|}  \\<in> set evso |]
-          ==> Notes Spy {|Nonce NA, Nonce NB, Key K|} # evso \\<in> yahalom"
+                             X|}  \<in> set evso |]
+          ==> Notes Spy {|Nonce NA, Nonce NB, Key K|} # evso \<in> yahalom"
+
+
+declare Says_imp_knows_Spy [THEN analz.Inj, dest]
+declare parts.Body  [dest]
+declare Fake_parts_insert_in_Un  [dest]
+declare analz_into_parts [dest]
+
+(*A "possibility property": there are traces that reach the end*)
+lemma "\<exists>X NB K. \<exists>evs \<in> yahalom.
+             Says A B {|X, Crypt K (Nonce NB)|} \<in> set evs"
+apply (intro exI bexI)
+apply (rule_tac [2] yahalom.Nil
+                    [THEN yahalom.YM1, THEN yahalom.Reception,
+                     THEN yahalom.YM2, THEN yahalom.Reception,
+                     THEN yahalom.YM3, THEN yahalom.Reception,
+                     THEN yahalom.YM4])
+apply possibility
+done
+
+lemma Gets_imp_Says:
+     "[| Gets B X \<in> set evs; evs \<in> yahalom |] ==> \<exists>A. Says A B X \<in> set evs"
+by (erule rev_mp, erule yahalom.induct, auto)
+
+(*Must be proved separately for each protocol*)
+lemma Gets_imp_knows_Spy:
+     "[| Gets B X \<in> set evs; evs \<in> yahalom |]  ==> X \<in> knows Spy evs"
+by (blast dest!: Gets_imp_Says Says_imp_knows_Spy)
+
+declare Gets_imp_knows_Spy [THEN analz.Inj, dest]
+
+
+(**** Inductive proofs about yahalom ****)
+
+(** For reasoning about the encrypted portion of messages **)
+
+(*Lets us treat YM4 using a similar argument as for the Fake case.*)
+lemma YM4_analz_knows_Spy:
+     "[| Gets A {|NB, Crypt (shrK A) Y, X|} \<in> set evs;  evs \<in> yahalom |]
+      ==> X \<in> analz (knows Spy evs)"
+by blast
+
+lemmas YM4_parts_knows_Spy =
+       YM4_analz_knows_Spy [THEN analz_into_parts, standard]
+
+
+(** Theorems of the form X \<notin> parts (knows Spy evs) imply that NOBODY
+    sends messages containing X! **)
+
+(*Spy never sees a good agent's shared key!*)
+lemma Spy_see_shrK [simp]:
+     "evs \<in> yahalom ==> (Key (shrK A) \<in> parts (knows Spy evs)) = (A \<in> bad)"
+apply (erule yahalom.induct, force,
+       drule_tac [6] YM4_parts_knows_Spy, simp_all)
+apply blast+
+done
+
+lemma Spy_analz_shrK [simp]:
+     "evs \<in> yahalom ==> (Key (shrK A) \<in> analz (knows Spy evs)) = (A \<in> bad)"
+by auto
+
+lemma Spy_see_shrK_D [dest!]:
+     "[|Key (shrK A) \<in> parts (knows Spy evs);  evs \<in> yahalom|] ==> A \<in> bad"
+by (blast dest: Spy_see_shrK)
+
+(*Nobody can have used non-existent keys!  Needed to apply analz_insert_Key*)
+lemma new_keys_not_used [rule_format, simp]:
+ "evs \<in> yahalom ==> Key K \<notin> used evs --> K \<notin> keysFor (parts (knows Spy evs))"
+apply (erule yahalom.induct, force,
+       frule_tac [6] YM4_parts_knows_Spy, simp_all)
+(*Fake, YM3, YM4*)
+apply (blast dest!: keysFor_parts_insert)+
+done
+
+
+(*Describes the form of K when the Server sends this message.  Useful for
+  Oops as well as main secrecy property.*)
+lemma Says_Server_message_form:
+     "[| Says Server A {|nb', Crypt (shrK A) {|Agent B, Key K, na|}, X|}
+          \<in> set evs;  evs \<in> yahalom |]
+      ==> K \<notin> range shrK"
+by (erule rev_mp, erule yahalom.induct, simp_all)
+
+
+(****
+ The following is to prove theorems of the form
+
+          Key K \<in> analz (insert (Key KAB) (knows Spy evs)) ==>
+          Key K \<in> analz (knows Spy evs)
+
+ A more general formula must be proved inductively.
+****)
+
+(** Session keys are not used to encrypt other session keys **)
+
+lemma analz_image_freshK [rule_format]:
+ "evs \<in> yahalom ==>
+   \<forall>K KK. KK <= - (range shrK) -->
+          (Key K \<in> analz (Key`KK Un (knows Spy evs))) =
+          (K \<in> KK | Key K \<in> analz (knows Spy evs))"
+apply (erule yahalom.induct, force, frule_tac [7] Says_Server_message_form,
+       drule_tac [6] YM4_analz_knows_Spy)
+apply analz_freshK
+apply spy_analz
+done
+
+lemma analz_insert_freshK:
+     "[| evs \<in> yahalom;  KAB \<notin> range shrK |] ==>
+      Key K \<in> analz (insert (Key KAB) (knows Spy evs)) =
+      (K = KAB | Key K \<in> analz (knows Spy evs))"
+by (simp only: analz_image_freshK analz_image_freshK_simps)
+
+
+(*** The Key K uniquely identifies the Server's  message. **)
+
+lemma unique_session_keys:
+     "[| Says Server A
+          {|nb, Crypt (shrK A) {|Agent B, Key K, na|}, X|} \<in> set evs;
+        Says Server A'
+          {|nb', Crypt (shrK A') {|Agent B', Key K, na'|}, X'|} \<in> set evs;
+        evs \<in> yahalom |]
+     ==> A=A' & B=B' & na=na' & nb=nb'"
+apply (erule rev_mp, erule rev_mp)
+apply (erule yahalom.induct, simp_all)
+(*YM3, by freshness*)
+apply blast
+done
+
+
+(** Crucial secrecy property: Spy does not see the keys sent in msg YM3 **)
+
+lemma secrecy_lemma:
+     "[| A \<notin> bad;  B \<notin> bad;  evs \<in> yahalom |]
+      ==> Says Server A
+            {|nb, Crypt (shrK A) {|Agent B, Key K, na|},
+                  Crypt (shrK B) {|Agent A, Agent B, Key K, nb|}|}
+           \<in> set evs -->
+          Notes Spy {|na, nb, Key K|} \<notin> set evs -->
+          Key K \<notin> analz (knows Spy evs)"
+apply (erule yahalom.induct, force, frule_tac [7] Says_Server_message_form,
+       drule_tac [6] YM4_analz_knows_Spy)
+apply (simp_all add: pushes analz_insert_eq analz_insert_freshK)
+apply spy_analz  (*Fake*)
+apply (blast dest: unique_session_keys)+  (*YM3, Oops*)
+done
+
+
+(*Final version*)
+lemma Spy_not_see_encrypted_key:
+     "[| Says Server A
+            {|nb, Crypt (shrK A) {|Agent B, Key K, na|},
+                  Crypt (shrK B) {|Agent A, Agent B, Key K, nb|}|}
+         \<in> set evs;
+         Notes Spy {|na, nb, Key K|} \<notin> set evs;
+         A \<notin> bad;  B \<notin> bad;  evs \<in> yahalom |]
+      ==> Key K \<notin> analz (knows Spy evs)"
+by (blast dest: secrecy_lemma Says_Server_message_form)
+
+
+(** Security Guarantee for A upon receiving YM3 **)
+
+(*If the encrypted message appears then it originated with the Server.
+  May now apply Spy_not_see_encrypted_key, subject to its conditions.*)
+lemma A_trusts_YM3:
+     "[| Crypt (shrK A) {|Agent B, Key K, na|} \<in> parts (knows Spy evs);
+         A \<notin> bad;  evs \<in> yahalom |]
+      ==> \<exists>nb. Says Server A
+                    {|nb, Crypt (shrK A) {|Agent B, Key K, na|},
+                          Crypt (shrK B) {|Agent A, Agent B, Key K, nb|}|}
+                  \<in> set evs"
+apply (erule rev_mp)
+apply (erule yahalom.induct, force,
+       frule_tac [6] YM4_parts_knows_Spy, simp_all)
+(*Fake, YM3*)
+apply blast+
+done
+
+(*The obvious combination of A_trusts_YM3 with Spy_not_see_encrypted_key*)
+lemma A_gets_good_key:
+     "[| Crypt (shrK A) {|Agent B, Key K, na|} \<in> parts (knows Spy evs);
+         \<forall>nb. Notes Spy {|na, nb, Key K|} \<notin> set evs;
+         A \<notin> bad;  B \<notin> bad;  evs \<in> yahalom |]
+      ==> Key K \<notin> analz (knows Spy evs)"
+by (blast dest!: A_trusts_YM3 Spy_not_see_encrypted_key)
+
+
+(** Security Guarantee for B upon receiving YM4 **)
+
+(*B knows, by the first part of A's message, that the Server distributed
+  the key for A and B, and has associated it with NB.*)
+lemma B_trusts_YM4_shrK:
+     "[| Crypt (shrK B) {|Agent A, Agent B, Key K, Nonce NB|}
+           \<in> parts (knows Spy evs);
+         B \<notin> bad;  evs \<in> yahalom |]
+  ==> \<exists>NA. Says Server A
+             {|Nonce NB,
+               Crypt (shrK A) {|Agent B, Key K, Nonce NA|},
+               Crypt (shrK B) {|Agent A, Agent B, Key K, Nonce NB|}|}
+             \<in> set evs"
+apply (erule rev_mp)
+apply (erule yahalom.induct, force,
+       frule_tac [6] YM4_parts_knows_Spy, simp_all)
+(*Fake, YM3*)
+apply blast+
+done
+
+
+(*With this protocol variant, we don't need the 2nd part of YM4 at all:
+  Nonce NB is available in the first part.*)
+
+(*What can B deduce from receipt of YM4?  Stronger and simpler than Yahalom
+  because we do not have to show that NB is secret. *)
+lemma B_trusts_YM4:
+     "[| Gets B {|Crypt (shrK B) {|Agent A, Agent B, Key K, Nonce NB|},  X|}
+           \<in> set evs;
+         A \<notin> bad;  B \<notin> bad;  evs \<in> yahalom |]
+  ==> \<exists>NA. Says Server A
+             {|Nonce NB,
+               Crypt (shrK A) {|Agent B, Key K, Nonce NA|},
+               Crypt (shrK B) {|Agent A, Agent B, Key K, Nonce NB|}|}
+            \<in> set evs"
+by (blast dest!: B_trusts_YM4_shrK)
+
+
+(*The obvious combination of B_trusts_YM4 with Spy_not_see_encrypted_key*)
+lemma B_gets_good_key:
+     "[| Gets B {|Crypt (shrK B) {|Agent A, Agent B, Key K, Nonce NB|}, X|}
+           \<in> set evs;
+         \<forall>na. Notes Spy {|na, Nonce NB, Key K|} \<notin> set evs;
+         A \<notin> bad;  B \<notin> bad;  evs \<in> yahalom |]
+      ==> Key K \<notin> analz (knows Spy evs)"
+by (blast dest!: B_trusts_YM4 Spy_not_see_encrypted_key)
+
+
+(*** Authenticating B to A ***)
+
+(*The encryption in message YM2 tells us it cannot be faked.*)
+lemma B_Said_YM2:
+     "[| Crypt (shrK B) {|Agent A, Nonce NA|} \<in> parts (knows Spy evs);
+         B \<notin> bad;  evs \<in> yahalom |]
+      ==> \<exists>NB. Says B Server {|Agent B, Nonce NB,
+                               Crypt (shrK B) {|Agent A, Nonce NA|}|}
+                      \<in> set evs"
+apply (erule rev_mp)
+apply (erule yahalom.induct, force,
+       frule_tac [6] YM4_parts_knows_Spy, simp_all)
+(*Fake, YM2*)
+apply blast+
+done
+
+
+(*If the server sends YM3 then B sent YM2, perhaps with a different NB*)
+lemma YM3_auth_B_to_A_lemma:
+     "[| Says Server A {|nb, Crypt (shrK A) {|Agent B, Key K, Nonce NA|}, X|}
+           \<in> set evs;
+         B \<notin> bad;  evs \<in> yahalom |]
+      ==> \<exists>nb'. Says B Server {|Agent B, nb',
+                                   Crypt (shrK B) {|Agent A, Nonce NA|}|}
+                       \<in> set evs"
+apply (erule rev_mp)
+apply (erule yahalom.induct, simp_all)
+(*Fake, YM2, YM3*)
+apply (blast dest!: B_Said_YM2)+
+done
+
+(*If A receives YM3 then B has used nonce NA (and therefore is alive)*)
+lemma YM3_auth_B_to_A:
+     "[| Gets A {|nb, Crypt (shrK A) {|Agent B, Key K, Nonce NA|}, X|}
+           \<in> set evs;
+         A \<notin> bad;  B \<notin> bad;  evs \<in> yahalom |]
+ ==> \<exists>nb'. Says B Server
+                  {|Agent B, nb', Crypt (shrK B) {|Agent A, Nonce NA|}|}
+               \<in> set evs"
+by (blast dest!: A_trusts_YM3 YM3_auth_B_to_A_lemma)
+
+
+
+(*** Authenticating A to B using the certificate Crypt K (Nonce NB) ***)
+
+(*Assuming the session key is secure, if both certificates are present then
+  A has said NB.  We can't be sure about the rest of A's message, but only
+  NB matters for freshness.  Note that  Key K \<notin> analz (knows Spy evs)  must be
+  the FIRST antecedent of the induction formula.*)
+
+(*This lemma allows a use of unique_session_keys in the next proof,
+  which otherwise is extremely slow.*)
+lemma secure_unique_session_keys:
+     "[| Crypt (shrK A) {|Agent B, Key K, na|} \<in> analz (spies evs);
+         Crypt (shrK A') {|Agent B', Key K, na'|} \<in> analz (spies evs);
+         Key K \<notin> analz (knows Spy evs);  evs \<in> yahalom |]
+     ==> A=A' & B=B'"
+by (blast dest!: A_trusts_YM3 dest: unique_session_keys Crypt_Spy_analz_bad)
+
+
+lemma Auth_A_to_B_lemma [rule_format]:
+     "evs \<in> yahalom
+      ==> Key K \<notin> analz (knows Spy evs) -->
+          Crypt K (Nonce NB) \<in> parts (knows Spy evs) -->
+          Crypt (shrK B) {|Agent A, Agent B, Key K, Nonce NB|}
+            \<in> parts (knows Spy evs) -->
+          B \<notin> bad -->
+          (\<exists>X. Says A B {|X, Crypt K (Nonce NB)|} \<in> set evs)"
+apply (erule yahalom.induct, force,
+       frule_tac [6] YM4_parts_knows_Spy)
+apply (analz_mono_contra, simp_all)
+(*Fake*)
+apply blast
+(*YM3: by new_keys_not_used we note that Crypt K (Nonce NB) could not exist*)
+apply (force dest!: Crypt_imp_keysFor)
+(*YM4: was Crypt K (Nonce NB) the very last message?  If so, apply unicity
+  of session keys; if not, use ind. hyp.*)
+apply (blast dest!: B_trusts_YM4_shrK dest: secure_unique_session_keys  )
+done
+
+
+(*If B receives YM4 then A has used nonce NB (and therefore is alive).
+  Moreover, A associates K with NB (thus is talking about the same run).
+  Other premises guarantee secrecy of K.*)
+lemma YM4_imp_A_Said_YM3 [rule_format]:
+     "[| Gets B {|Crypt (shrK B) {|Agent A, Agent B, Key K, Nonce NB|},
+                  Crypt K (Nonce NB)|} \<in> set evs;
+         (\<forall>NA. Notes Spy {|Nonce NA, Nonce NB, Key K|} \<notin> set evs);
+         A \<notin> bad;  B \<notin> bad;  evs \<in> yahalom |]
+      ==> \<exists>X. Says A B {|X, Crypt K (Nonce NB)|} \<in> set evs"
+by (blast intro: Auth_A_to_B_lemma
+          dest: Spy_not_see_encrypted_key B_trusts_YM4_shrK)
 
 end
