src/HOL/Auth/Yahalom_Bad.thy
@@ -5,62 +5,354 @@
 
 Inductive relation "yahalom" for the Yahalom protocol.
 
-Example of why Oops is necessary.  This protocol can be attacked because it
-doesn't keep NB secret, but without Oops it can be "verified" anyway.
+Demonstrates of why Oops is necessary.  This protocol can be attacked because
+it doesn't keep NB secret, but without Oops it can be "verified" anyway.
+The issues are discussed in lcp's LICS 2000 invited lecture.
 *)
 
-Yahalom_Bad = Shared + 
+theory Yahalom_Bad = Shared:
 
-consts  yahalom   :: event list set
+consts  yahalom   :: "event list set"
 inductive "yahalom"
-  intrs 
+  intros
          (*Initial trace is empty*)
-    Nil  "[] : yahalom"
+   Nil:  "[] \<in> yahalom"
 
          (*The spy MAY say anything he CAN say.  We do not expect him to
            invent new nonces here, but he can also use NS1.  Common to
            all similar protocols.*)
-    Fake "[| evsf \\<in> yahalom;  X \\<in> synth (analz (knows Spy evsf)) |]
-          ==> Says Spy B X  # evsf \\<in> yahalom"
+   Fake: "[| evsf \<in> yahalom;  X \<in> synth (analz (knows Spy evsf)) |]
+          ==> Says Spy B X  # evsf \<in> yahalom"
 
          (*A message that has been sent can be received by the
            intended recipient.*)
-    Reception "[| evsr \\<in> yahalom;  Says A B X \\<in> set evsr |]
-               ==> Gets B X # evsr \\<in> yahalom"
+   Reception: "[| evsr \<in> yahalom;  Says A B X \<in> set evsr |]
+               ==> Gets B X # evsr \<in> yahalom"
 
          (*Alice initiates a protocol run*)
-    YM1  "[| evs1 \\<in> yahalom;  Nonce NA \\<notin> used evs1 |]
-          ==> Says A B {|Agent A, Nonce NA|} # evs1 \\<in> yahalom"
+   YM1:  "[| evs1 \<in> yahalom;  Nonce NA \<notin> used evs1 |]
+          ==> Says A B {|Agent A, Nonce NA|} # evs1 \<in> yahalom"
 
          (*Bob's response to Alice's message.*)
-    YM2  "[| evs2 \\<in> yahalom;  Nonce NB \\<notin> used evs2;
-             Gets B {|Agent A, Nonce NA|} \\<in> set evs2 |]
-          ==> Says B Server 
+   YM2:  "[| evs2 \<in> yahalom;  Nonce NB \<notin> used evs2;
+             Gets B {|Agent A, Nonce NA|} \<in> set evs2 |]
+          ==> Says B Server
                   {|Agent B, Nonce NB, Crypt (shrK B) {|Agent A, Nonce NA|}|}
-                # evs2 \\<in> yahalom"
+                # evs2 \<in> yahalom"
 
          (*The Server receives Bob's message.  He responds by sending a
             new session key to Alice, with a packet for forwarding to Bob.*)
-    YM3  "[| evs3 \\<in> yahalom;  Key KAB \\<notin> used evs3;
-             Gets Server 
+   YM3:  "[| evs3 \<in> yahalom;  Key KAB \<notin> used evs3;
+             Gets Server
                   {|Agent B, Nonce NB, Crypt (shrK B) {|Agent A, Nonce NA|}|}
-               \\<in> set evs3 |]
+               \<in> set evs3 |]
           ==> Says Server A
                    {|Crypt (shrK A) {|Agent B, Key KAB, Nonce NA, Nonce NB|},
                      Crypt (shrK B) {|Agent A, Key KAB|}|}
-                # evs3 \\<in> yahalom"
+                # evs3 \<in> yahalom"
 
          (*Alice receives the Server's (?) message, checks her Nonce, and
            uses the new session key to send Bob his Nonce.  The premise
-           A \\<noteq> Server is needed to prove Says_Server_not_range.*)
-    YM4  "[| evs4 \\<in> yahalom;  A \\<noteq> Server;
+           A \<noteq> Server is needed to prove Says_Server_not_range.*)
+   YM4:  "[| evs4 \<in> yahalom;  A \<noteq> Server;
              Gets A {|Crypt(shrK A) {|Agent B, Key K, Nonce NA, Nonce NB|}, X|}
-                \\<in> set evs4;
-             Says A B {|Agent A, Nonce NA|} \\<in> set evs4 |]
-          ==> Says A B {|X, Crypt K (Nonce NB)|} # evs4 \\<in> yahalom"
+                \<in> set evs4;
+             Says A B {|Agent A, Nonce NA|} \<in> set evs4 |]
+          ==> Says A B {|X, Crypt K (Nonce NB)|} # evs4 \<in> yahalom"
 
-         (*This message models possible leaks of session keys.  The Nonces
-           identify the protocol run.  Quoting Server here ensures they are
-           correct.*)
+
+declare Says_imp_knows_Spy [THEN analz.Inj, dest]
+declare parts.Body  [dest]
+declare Fake_parts_insert_in_Un  [dest]
+declare analz_into_parts [dest]
+
+
+(*A "possibility property": there are traces that reach the end*)
+lemma "A \<noteq> Server
+      ==> \<exists>X NB K. \<exists>evs \<in> yahalom.
+             Says A B {|X, Crypt K (Nonce NB)|} \<in> set evs"
+apply (intro exI bexI)
+apply (rule_tac [2] yahalom.Nil
+                    [THEN yahalom.YM1, THEN yahalom.Reception,
+                     THEN yahalom.YM2, THEN yahalom.Reception,
+                     THEN yahalom.YM3, THEN yahalom.Reception,
+                     THEN yahalom.YM4])
+apply possibility
+done
+
+lemma Gets_imp_Says:
+     "[| Gets B X \<in> set evs; evs \<in> yahalom |] ==> \<exists>A. Says A B X \<in> set evs"
+by (erule rev_mp, erule yahalom.induct, auto)
+
+(*Must be proved separately for each protocol*)
+lemma Gets_imp_knows_Spy:
+     "[| Gets B X \<in> set evs; evs \<in> yahalom |]  ==> X \<in> knows Spy evs"
+by (blast dest!: Gets_imp_Says Says_imp_knows_Spy)
+
+declare Gets_imp_knows_Spy [THEN analz.Inj, dest]
+
+
+(**** Inductive proofs about yahalom ****)
+
+(** For reasoning about the encrypted portion of messages **)
+
+(*Lets us treat YM4 using a similar argument as for the Fake case.*)
+lemma YM4_analz_knows_Spy:
+     "[| Gets A {|Crypt (shrK A) Y, X|} \<in> set evs;  evs \<in> yahalom |]
+      ==> X \<in> analz (knows Spy evs)"
+by blast
+
+lemmas YM4_parts_knows_Spy =
+       YM4_analz_knows_Spy [THEN analz_into_parts, standard]
+
+
+(** Theorems of the form X \<notin> parts (knows Spy evs) imply that NOBODY
+    sends messages containing X! **)
+
+(*Spy never sees a good agent's shared key!*)
+lemma Spy_see_shrK [simp]:
+     "evs \<in> yahalom ==> (Key (shrK A) \<in> parts (knows Spy evs)) = (A \<in> bad)"
+apply (erule yahalom.induct, force,
+       drule_tac [6] YM4_parts_knows_Spy, simp_all)
+apply blast+
+done
+
+lemma Spy_analz_shrK [simp]:
+     "evs \<in> yahalom ==> (Key (shrK A) \<in> analz (knows Spy evs)) = (A \<in> bad)"
+by auto
+
+lemma Spy_see_shrK_D [dest!]:
+     "[|Key (shrK A) \<in> parts (knows Spy evs);  evs \<in> yahalom|] ==> A \<in> bad"
+by (blast dest: Spy_see_shrK)
+
+(*Nobody can have used non-existent keys!  Needed to apply analz_insert_Key*)
+lemma new_keys_not_used [rule_format, simp]:
+ "evs \<in> yahalom ==> Key K \<notin> used evs --> K \<notin> keysFor (parts (knows Spy evs))"
+apply (erule yahalom.induct, force,
+       frule_tac [6] YM4_parts_knows_Spy, simp_all)
+(*Fake, YM3, YM4*)
+apply (blast dest!: keysFor_parts_insert)+
+done
+
+
+(****
+ The following is to prove theorems of the form
+
+  Key K \<in> analz (insert (Key KAB) (knows Spy evs)) ==>
+  Key K \<in> analz (knows Spy evs)
+
+ A more general formula must be proved inductively.
+****)
+
+(** Session keys are not used to encrypt other session keys **)
+
+lemma analz_image_freshK [rule_format]:
+ "evs \<in> yahalom ==>
+   \<forall>K KK. KK <= - (range shrK) -->
+          (Key K \<in> analz (Key`KK Un (knows Spy evs))) =
+          (K \<in> KK | Key K \<in> analz (knows Spy evs))"
+apply (erule yahalom.induct, force,
+       drule_tac [6] YM4_analz_knows_Spy)
+apply analz_freshK
+apply spy_analz
+done
+
+lemma analz_insert_freshK: "[| evs \<in> yahalom;  KAB \<notin> range shrK |] ==>
+      Key K \<in> analz (insert (Key KAB) (knows Spy evs)) =
+      (K = KAB | Key K \<in> analz (knows Spy evs))"
+by (simp only: analz_image_freshK analz_image_freshK_simps)
+
+
+(*** The Key K uniquely identifies the Server's  message. **)
+
+lemma unique_session_keys:
+     "[| Says Server A
+          {|Crypt (shrK A) {|Agent B, Key K, na, nb|}, X|} \<in> set evs;
+        Says Server A'
+          {|Crypt (shrK A') {|Agent B', Key K, na', nb'|}, X'|} \<in> set evs;
+        evs \<in> yahalom |]
+     ==> A=A' & B=B' & na=na' & nb=nb'"
+apply (erule rev_mp, erule rev_mp)
+apply (erule yahalom.induct, simp_all)
+(*YM3, by freshness, and YM4*)
+apply blast+
+done
+
+
+(** Crucial secrecy property: Spy does not see the keys sent in msg YM3 **)
+
+lemma secrecy_lemma:
+     "[| A \<notin> bad;  B \<notin> bad;  evs \<in> yahalom |]
+      ==> Says Server A
+            {|Crypt (shrK A) {|Agent B, Key K, na, nb|},
+              Crypt (shrK B) {|Agent A, Key K|}|}
+           \<in> set evs -->
+          Key K \<notin> analz (knows Spy evs)"
+apply (erule yahalom.induct, force, drule_tac [6] YM4_analz_knows_Spy)
+apply (simp_all add: pushes analz_insert_eq analz_insert_freshK)
+apply spy_analz  (*Fake*)
+apply (blast dest: unique_session_keys)  (*YM3*)
+done
+
+(*Final version*)
+lemma Spy_not_see_encrypted_key:
+     "[| Says Server A
+            {|Crypt (shrK A) {|Agent B, Key K, na, nb|},
+              Crypt (shrK B) {|Agent A, Key K|}|}
+           \<in> set evs;
+         A \<notin> bad;  B \<notin> bad;  evs \<in> yahalom |]
+      ==> Key K \<notin> analz (knows Spy evs)"
+by (blast dest: secrecy_lemma)
+
+
+(** Security Guarantee for A upon receiving YM3 **)
+
+(*If the encrypted message appears then it originated with the Server*)
+lemma A_trusts_YM3:
+     "[| Crypt (shrK A) {|Agent B, Key K, na, nb|} \<in> parts (knows Spy evs);
+         A \<notin> bad;  evs \<in> yahalom |]
+       ==> Says Server A
+            {|Crypt (shrK A) {|Agent B, Key K, na, nb|},
+              Crypt (shrK B) {|Agent A, Key K|}|}
+           \<in> set evs"
+apply (erule rev_mp)
+apply (erule yahalom.induct, force,
+       frule_tac [6] YM4_parts_knows_Spy, simp_all)
+(*Fake, YM3*)
+apply blast+
+done
+
+(*The obvious combination of A_trusts_YM3 with Spy_not_see_encrypted_key*)
+lemma A_gets_good_key:
+     "[| Crypt (shrK A) {|Agent B, Key K, na, nb|} \<in> parts (knows Spy evs);
+         A \<notin> bad;  B \<notin> bad;  evs \<in> yahalom |]
+      ==> Key K \<notin> analz (knows Spy evs)"
+by (blast dest!: A_trusts_YM3 Spy_not_see_encrypted_key)
+
+(** Security Guarantees for B upon receiving YM4 **)
+
+(*B knows, by the first part of A's message, that the Server distributed
+  the key for A and B.  But this part says nothing about nonces.*)
+lemma B_trusts_YM4_shrK:
+     "[| Crypt (shrK B) {|Agent A, Key K|} \<in> parts (knows Spy evs);
+         B \<notin> bad;  evs \<in> yahalom |]
+      ==> \<exists>NA NB. Says Server A
+                      {|Crypt (shrK A) {|Agent B, Key K, Nonce NA, Nonce NB|},
+                        Crypt (shrK B) {|Agent A, Key K|}|}
+                     \<in> set evs"
+apply (erule rev_mp)
+apply (erule yahalom.induct, force,
+       frule_tac [6] YM4_parts_knows_Spy, simp_all)
+(*Fake, YM3*)
+apply blast+
+done
+
+(** Up to now, the reasoning is similar to standard Yahalom.  Now the
+    doubtful reasoning occurs.  We should not be assuming that an unknown
+    key is secure, but the model allows us to: there is no Oops rule to
+    let session keys become compromised.*)
+
+(*B knows, by the second part of A's message, that the Server distributed
+  the key quoting nonce NB.  This part says nothing about agent names.
+  Secrecy of K is assumed; the valid Yahalom proof uses (and later proves)
+  the secrecy of NB.*)
+lemma B_trusts_YM4_newK [rule_format]:
+     "[|Key K \<notin> analz (knows Spy evs);  evs \<in> yahalom|]
+      ==> Crypt K (Nonce NB) \<in> parts (knows Spy evs) -->
+          (\<exists>A B NA. Says Server A
+                      {|Crypt (shrK A) {|Agent B, Key K,
+                                Nonce NA, Nonce NB|},
+                        Crypt (shrK B) {|Agent A, Key K|}|}
+                     \<in> set evs)"
+apply (erule rev_mp)
+apply (erule yahalom.induct, force,
+       frule_tac [6] YM4_parts_knows_Spy)
+apply (analz_mono_contra, simp_all)
+(*Fake*)
+apply blast
+(*YM3*)
+apply blast
+(*A is uncompromised because NB is secure
+  A's certificate guarantees the existence of the Server message*)
+apply (blast dest!: Gets_imp_Says Crypt_Spy_analz_bad
+             dest: Says_imp_spies
+                   parts.Inj [THEN parts.Fst, THEN A_trusts_YM3])
+done
+
+
+(*B's session key guarantee from YM4.  The two certificates contribute to a
+  single conclusion about the Server's message. *)
+lemma B_trusts_YM4:
+     "[| Gets B {|Crypt (shrK B) {|Agent A, Key K|},
+                  Crypt K (Nonce NB)|} \<in> set evs;
+         Says B Server
+           {|Agent B, Nonce NB, Crypt (shrK B) {|Agent A, Nonce NA|}|}
+           \<in> set evs;
+         A \<notin> bad;  B \<notin> bad;  evs \<in> yahalom |]
+       ==> \<exists>na nb. Says Server A
+                   {|Crypt (shrK A) {|Agent B, Key K, na, nb|},
+                     Crypt (shrK B) {|Agent A, Key K|}|}
+             \<in> set evs"
+by (blast dest: B_trusts_YM4_newK B_trusts_YM4_shrK Spy_not_see_encrypted_key
+                unique_session_keys)
+
+
+(*The obvious combination of B_trusts_YM4 with Spy_not_see_encrypted_key*)
+lemma B_gets_good_key:
+     "[| Gets B {|Crypt (shrK B) {|Agent A, Key K|},
+                  Crypt K (Nonce NB)|} \<in> set evs;
+         Says B Server
+           {|Agent B, Nonce NB, Crypt (shrK B) {|Agent A, Nonce NA|}|}
+           \<in> set evs;
+         A \<notin> bad;  B \<notin> bad;  evs \<in> yahalom |]
+      ==> Key K \<notin> analz (knows Spy evs)"
+by (blast dest!: B_trusts_YM4 Spy_not_see_encrypted_key)
+
+
+(*** Authenticating B to A: these proofs are not considered.
+     They are irrelevant to showing the need for Oops. ***)
+
+
+(*** Authenticating A to B using the certificate Crypt K (Nonce NB) ***)
+
+(*Assuming the session key is secure, if both certificates are present then
+  A has said NB.  We can't be sure about the rest of A's message, but only
+  NB matters for freshness.*)
+lemma A_Said_YM3_lemma [rule_format]:
+     "evs \<in> yahalom
+      ==> Key K \<notin> analz (knows Spy evs) -->
+          Crypt K (Nonce NB) \<in> parts (knows Spy evs) -->
+          Crypt (shrK B) {|Agent A, Key K|} \<in> parts (knows Spy evs) -->
+          B \<notin> bad -->
+          (\<exists>X. Says A B {|X, Crypt K (Nonce NB)|} \<in> set evs)"
+apply (erule yahalom.induct, force,
+       frule_tac [6] YM4_parts_knows_Spy)
+apply (analz_mono_contra, simp_all)
+(*Fake*)
+apply blast
+(*YM3: by new_keys_not_used we note that Crypt K (Nonce NB) could not exist*)
+apply (force dest!: Crypt_imp_keysFor)
+(*YM4: was Crypt K (Nonce NB) the very last message?  If not, use ind. hyp.*)
+apply (simp add: ex_disj_distrib)
+(*yes: apply unicity of session keys*)
+apply (blast dest!: Gets_imp_Says A_trusts_YM3 B_trusts_YM4_shrK
+                    Crypt_Spy_analz_bad
+             dest: Says_imp_knows_Spy [THEN parts.Inj] unique_session_keys)
+done
+
+(*If B receives YM4 then A has used nonce NB (and therefore is alive).
+  Moreover, A associates K with NB (thus is talking about the same run).
+  Other premises guarantee secrecy of K.*)
+lemma YM4_imp_A_Said_YM3 [rule_format]:
+     "[| Gets B {|Crypt (shrK B) {|Agent A, Key K|},
+                  Crypt K (Nonce NB)|} \<in> set evs;
+         Says B Server
+           {|Agent B, Nonce NB, Crypt (shrK B) {|Agent A, Nonce NA|}|}
+           \<in> set evs;
+         A \<notin> bad;  B \<notin> bad;  evs \<in> yahalom |]
+      ==> \<exists>X. Says A B {|X, Crypt K (Nonce NB)|} \<in> set evs"
+apply (blast intro!: A_Said_YM3_lemma
+            dest: Spy_not_see_encrypted_key B_trusts_YM4 Gets_imp_Says)
+done
 
 end
